<section xml:id="sec_inverse-trig-hyperbolics">
  <title>Inverse Trigonometric and Hyperbolic Functions</title>
  <p>
    We expressed trigonometric and hyperbolic functions in Section 5.4 in terms of the exponential function.
    In this section we look at their inverses.
    When we solve equations such as <m>w=\sin z</m> for <m>z</m>,
    we obtain formulas that involve the logarithm.
    Because trigonometric and hyperbolic functions are all periodic,
    they are many-to-one;
    hence their inverses are necessarily multivalued.
    The formulas for the inverse trigonometric functions are
    <md>
      <mrow xml:id="arcsinz" number="yes">\arcsin z \amp = -i\log \left[ iz+( 1-z^2 )^{\frac{1}{2}}\right],</mrow>
      <mrow>\arccos z \amp = -i\log \left[ z+i( 1-z^2 )^{\frac{1}{2}}\right],  \text{ and }</mrow>
      <mrow>\arctan z \amp = \frac{i}{2}\log(\frac{i+z}{i-z})</mrow>
    </md>.
  </p>
  <p>
    We can find the derivatives of any branch of these functions by using the chain rule:
    <md>
      <mrow xml:id="Deriv_arcsinz" number="yes">\frac{d}{dz}\arcsin z \amp = \frac{1}{( 1-z^2 )^{\frac{1}{2}}},</mrow>
      <mrow>\frac{d}{dz}\arccos z \amp = \frac{-1}{( 1-z^2 )^{\frac{1}{2}}},  \text{ and }</mrow>
      <mrow>\frac{d}{dz}\arctan z \amp = \frac{1}{1+z^2 }</mrow>
    </md>.
  </p>
  <p>
    We derive Equations <xref ref="arcsinz"/> and <xref ref="Deriv_arcsinz"/> and leave the others as exercises.
    If we take a particular branch of the multivalued function,
    <m>w=\arcsin z</m>, we have
    <me>
      z=\sin w=\frac{1}{2i}( e^{iw}-e^{-iw})
    </me>,
    which we can also write as
    <me>
      e^{iw}-2iz-e^{-iw}=0
    </me>.
  </p>
  <p>
    Multiplying both sides of this equation by <m>e^{iw}</m> gives <m>(e^{iw})^2 -2ize^{iw}-1=0</m>,
    which is a quadratic equation in terms of <m>e^{iw}</m>.
    Using the quadratic equation to solve for <m>e^{iw}</m>,
    we obtain
    <me>
      e^{iw}=\frac{2iz+( 4-4z^2 )^{\frac{1}{2}}}{2}=iz+(1-z^2 )^{\frac{1}{2}}
    </me>,
    where the square root is a multivalued function.
    Taking the logarithm of both sides of this last equation leads to the desired result:
    <me>
      w=\arcsin z=-i\log \left[ iz+( 1-z^2 )^{\frac{1}{2}}\right]
    </me>.
    where the multivalued logarithm is used.
    To construct a specific branch of <m>\arcsin z</m>,
    we must first select a branch of the square root and then select a branch of the logarithm.
  </p>
  <p>
    We get the derivative of <m>w=\arcsin z</m> by starting with the equation
    <m>\sin w=z</m> and differentiating both sides, using the chain rule:
    <md>
      <mrow>\frac{d}{dz}\sin w        \amp = \frac{d}{dz}z,</mrow>
      <mrow>\frac{d}{dw}\sin w\frac{dw}{dz} \amp = 1,</mrow>
      <mrow>\frac{dw}{dz}          \amp = \frac{1}{\cos w}</mrow>
    </md>.
  </p>
  <p>
    When the principal value is used,
    <m>w=\arcsin z=-i\mathrm{Log}\left[ iz+( 1-z^2 )^{\frac{1}{2}}\right]</m> maps the upper half-plane
    <m>\{z:\mathrm{Im}(z) >0\}</m> onto a portion of the upper half-plane
    <m>\{w:\mathrm{Im}( w) >0\}</m> that lies in the vertical strip <m>\{w:\frac{-\pi }{2}\lt \mathrm{Re}( w) \lt \frac{\pi }{2}\}</m>.
    The image of a rectangular grid in the <m>z</m> plane is a
    <q>spider web</q>
    in the <m>w</m> plane, as <xref ref="fig_ch-05-10">Figure</xref> shows.
  </p>
  <figure xml:id="fig_ch-05-10">
    <caption>A rectangular grid is mapped onto a spider web by <m>w=\arcsin z</m></caption>
    <image width="73%" source="figs/ch-05/ch-05-fig-10.pdf"/>
  </figure>
  <example>
    <statement>
      <p>
        The values of <m>\arcsin \sqrt{2}</m> are given by
        <men xml:id="arcsin_root2_">
          \arcsin \sqrt{2} = -i\log \left[ i\sqrt{2}+ \left( 1-\left(\sqrt{2}\right)^2\right)^{\frac{1}{2}}\right] =-i\log(i\sqrt{2}\pm i)
        </men>.
      </p>
      <p>
        Using straightforward techniques,
        we simplify this equation and obtain
        <md>
          <mrow>\arcsin \sqrt{2}  \amp = -i\log \left[(\sqrt{2}\pm 1) i\right]</mrow>
          <mrow>\amp = i\left[ \ln(\sqrt{2}\pm 1) +i\left(\frac{\pi }{2}+2n\pi\right)\right]</mrow>
          <mrow>\amp = \frac{\pi }{2}+2n\pi -i\ln(\sqrt{2}\pm 1),  \text{ where }  n \text{ is an integer. }</mrow>
        </md>
      </p>
      <p>
        We observe that
        <me>
          \ln(\sqrt{2}-1) =\ln \frac{( \sqrt{2}-1)(\sqrt{2}+1) }{\sqrt{2}+1}=\ln \frac{1}{\sqrt{2}+1}=-\ln(\sqrt{2}+1)
        </me>
        and then write
        <me>
          \arcsin \sqrt{2}=\frac{\pi }{2}+2n\pi \pm i\ln(\sqrt{2}+1),  \text{ where }  n \text{ is an integer }
        </me>.
      </p>
    </statement>
  </example>
  <example>
    <statement>
      <p>
        Suppose that we make specific choices in Equation <xref ref="arcsin_root2_"/> by selecting <m>+i</m> as the value of the square root
        <m>[1-(\sqrt{2})^2]^{\frac{1}{2}}</m> and using the principal value of the logarithm.
        With <m>f(z) =\mathrm{Arcsin}\,z</m>, The result is
        <me>
          f(\sqrt{2}) =\mathrm{Arcsin}\sqrt{2}=-i\mathrm{Log}( i\sqrt{2}+i) =\frac{\pi }{2}-i\ln(\sqrt{2}+1)
        </me>,
        and the corresponding value of the derivative is given by
        <me>
          f\,'( \sqrt{2}) =\frac{1}{\left[ 1-\left(\sqrt{2}\right)^2 \right]^{\frac{1}{2}}}=\frac{1}{i}=-i
        </me>.
      </p>
    </statement>
  </example>
  <p>
    The inverse hyperbolic functions are
    <md>
      <mrow>\text{ arcsinh\ } z \amp = \log \left[ z+(z^2 +1)^{\frac{1}{2}} \right],</mrow>
      <mrow>\text{ arccosh\ } z \amp = \log \left[ z+(z^2 -1)^{\frac{1}{2}} \right] \text{ , and }</mrow>
      <mrow xml:id="arctanhz" number="yes">\text{ arctanh\ } z \amp = \frac{1}{2}\log\left(\frac{1+z}{1-z}\right)</mrow>
    </md>.
  </p>
  <p>
    Their derivatives are
    <md>
      <mrow>\frac{d}{dz}\text{ arcsinh\ } z \amp = \frac{1}{(z^2 +1)^{\frac{1}{2}}},</mrow>
      <mrow>\frac{d}{dz}\text{ arccosh\ } z \amp = \frac{1}{(z^2 -1)^{\frac{1}{2}}},  \text{ and }</mrow>
      <mrow>\frac{d}{dz}\text{ arctanh\ } z \amp = \frac{1}{1-z^2 }</mrow>
    </md>.
  </p>
  <p>
    To establish <xref ref="arctanhz">Identity</xref>,
    we start with <m>w=</m> arctanh<m>z</m> and obtain
    <me>
      z=\tanh w=\frac{e^{w}-e^{-w}}{e^{w}+e^{-w}}=\frac{e^{2w}-1}{e^{2w}+1}
    </me>.
    which we solve for <m>e^{2w}</m>,
    getting <m>e^{2w}=\frac{1+z}{1-z}</m>.
    Taking the logarithms of both sides gives
    <me>
      w=\text{ arctanh\ } z=\frac{1}{2}\log\left(\frac{1+z}{1-z}\right)
    </me>,
    which is what we wanted to show.
  </p>
  <example>
    <statement>
      <p>
        Calculation reveals that
        <md>
          <mrow>\text{ arctanh } ( 1+2i)  \amp = \frac{1}{2}\log \frac{1+1+2i}{1-1-2i}=\frac{1}{2}\log(-1+i)</mrow>
          <mrow>\amp = \frac{1}{4}\ln 2+i\left(\frac{3}{8}+n\right)\pi</mrow>
        </md>,
        where <m>n</m> is an integer.
      </p>
    </statement>
  </example>
  <exercises>
    <title>Exercises for <xref ref="sec_inverse-trig-hyperbolics">Section</xref></title>
    <exercise xml:id="x5_5_1">
      <p>
        Find <em>all</em> values of the following.
      </p>
      <ol>
        <li>
          <p>
            <m>\arcsin \frac{5}{4}</m>.
          </p>
        </li>
        <li>
          <p>
            <m>\arccos \frac{5}{3}</m>.
          </p>
        </li>
        <li>
          <p>
            <m>\arcsin 3</m>.
          </p>
        </li>
        <li>
          <p>
            <m>\arccos 3i</m>.
          </p>
        </li>
        <li>
          <p>
            <m>\arctan 2i</m>.
          </p>
        </li>
        <li>
          <p>
            <m>\arctan i</m>.
          </p>
        </li>
        <li>
          <p>
            <m>\mathrm{arcsinh}\,i</m>.
          </p>
        </li>
        <li>
          <p>
            <m>\mathrm{arcsinh}\, \frac{3}{4}</m>.
          </p>
        </li>
        <li>
          <p>
            <m>\mathrm{arccosh}\, i</m>.
          </p>
        </li>
        <li>
          <p>
            <m>\mathrm{arccosh}\, \frac{1}{2}</m>.
          </p>
        </li>
        <li>
          <p>
            <m>\mathrm{arctanh}\, i</m>.
          </p>
        </li>
        <li>
          <p>
            <m>\mathrm{arctanh}\, i\sqrt{3}</m>.
          </p>
        </li>
      </ol>
    </exercise>
    <exercise xml:id="x5_5_2">
      <p>
        Establish the following identities .
        <ol>
          <li>
            <p>
              <m>\arccos z=-i\log \left[z+i( 1-z^2 )^{\frac{1}{2}}\right]</m>.
            </p>
          </li>
          <li>
            <p>
              <m>\frac{d}{dz}\arccos z=\frac{-1}{( 1-z^2 )^{\frac{1}{2}}}</m>.
            </p>
          </li>
          <li>
            <p>
              <m>\arctan z=\frac{i}{2}\log(\frac{i+z}{i-z})</m>.
            </p>
          </li>
          <li>
            <p>
              <m>\frac{d}{dz}\arctan z=\frac{1}{1+z^2 }</m>.
            </p>
          </li>
          <li xml:id="x5_5_2e">
            <p>
              <m>\arcsin z+\arccos z=\frac{\pi}{2}+2n\pi</m>,
              where <m>n</m> is an integer.
            </p>
          </li>
          <li>
            <p>
              <m>\frac{d}{dz}\mathrm{arctanh}\,z=\frac{1}{1-z^2}</m>.
            </p>
          </li>
          <li>
            <p>
              <m>\mathrm{arcsinh}\,z=\log \left[z+(z^2 +1)^{\frac{1}{2}}\right]</m>.
            </p>
          </li>
          <li>
            <p>
              <m>\frac{d}{dz}\mathrm{arcsinh}\,z=\frac{1}{(z^2 +1)^{1/2}}</m>.
            </p>
          </li>
          <li>
            <p>
              <m>\mathrm{arccosh}\,z=\log\left[ z+(z^2 -1)^{\frac{1}{2}}\right]</m>.
            </p>
          </li>
          <li>
            <p>
              <m>\frac{d}{dz}\mathrm{arccosh}\,z=\frac{1}{(z^2 -1)^{\frac{1}{2}}}</m>.
            </p>
          </li>
        </ol>
      </p>
    </exercise>
  </exercises>
</section>