<section xml:id="sec_improper-trig-integrals">
  <title>Improper Integrals of Trigonometric Functions</title>
  <p>
    Let <m>P</m> and <m>Q</m> be polynomials of degree <m>m</m> and <m>n</m>,
    respectively, where <m>n\ge m+1</m>.
    We can show
    (but omit the proof)
    that if <m>Q(x) \ne 0</m> for all real <m>x</m>, then
    <me>
      \text{ P.V. } \int_{-\infty}^{\infty}\frac{P(x)}{Q(x)}\cos x\,dx  \text{ and }   \text{ P.V. } \int_{-\infty}^{\infty}\frac{P(x)}{Q(x)}\sin x\,dx
    </me>
    are convergent improper integrals.
    You may encounter integrals of this type in the study of Fourier transforms and Fourier integrals.
    We now show how to evaluate them.
  </p>
  <p>
    Particularly important is our use of the identities
    <me>
      \cos(\alpha x) =\mathrm{Re}[\exp(i\alpha x)]  \text{ and }   \sin (\alpha x) =\mathrm{Im}[\exp (i\alpha x)]
    </me>,
    where <m>\alpha</m> is a positive real number.
    The crucial step in the proof of the following Theorem wouldn't hold if we were to use <m>\cos(\alpha z)</m> and
    <m>\sin (\alpha z)</m> instead of <m>\exp (i\alpha z)</m>,
    as you will see when you get to <xref ref="Jordan_s_Lemma">Lemma</xref>.
  </p>
  <theorem xml:id="PV_P_Q_sin__cos_thm">
    <statement>
      <p>
        Let <m>P</m><nbsp/>and <m>Q</m><nbsp/>be polynomials with real coefficients of degree <m>m</m><nbsp/>and <m>n</m>,
        respectively,
        where <m>n \ge m+1</m> and
        <m>Q(x) \ne 0</m>, for all real <m>x</m>.
        If <m>\alpha>0</m> and
        <men xml:id="exp_iaz_P_z__Q_z_">
          f(z) = \frac{\exp(i\alpha z)P(z)}{Q(z)}
        </men>.
        then
        <md>
          <mrow xml:id="PV__P_Q_cos_ax_" number="yes">\text{ P.V. }  \int_{-\infty}^{\infty}\frac{P(x)}{Q(x)}\cos(\alpha x)\,dx \amp = -2\pi\sum \limits_{j=1}^k \mathrm{Im}(\mathrm{Res}[f,z_j]),  \text{ and }</mrow>
          <mrow xml:id="PV__P_Q_sin_ax_" number="yes">\text{ P.V. } \int_{-\infty}^{\infty}\frac{P(x)}{Q(x)}\sin(\alpha x)\,dx \amp = 2\pi\sum \limits_{j=1}^k\mathrm{Re}(\mathrm{Res}[f,z_j])</mrow>
        </md>,
        where <m>z_1, \, z_2, \, \ldots, \, z_{k-1}, \, z_k</m> are the poles of <m>f</m> that lie in the upper half-plane,
        and <m>\mathrm{Re}(\mathrm{Res}[f,z_j])</m> and
        <m>\mathrm{Im}(\mathrm{Res}[f,z_j])</m> are the real and imaginary parts of <m>\mathrm{Res}[f,z_j]</m>,
        respectively.
      </p>
    </statement>
  </theorem>
  <p>
    The proof of <xref ref="PV_P_Q_sin__cos_thm">Theorem</xref>
    is similar to the proof of <xref ref="Ratl_Fcn_Int_Thm">Theorem</xref>.
    Before turning to the proof,
    we illustrate how to use <xref ref="PV_P_Q_sin__cos_thm">Theorem</xref>
  </p>
  <example>
    <statement>
      <p>
        Evaluate P.V. <m>\int_{-\infty}^{\infty}\frac{x\sin x}{x^2+4}\,dx</m>.
      </p>
      <p>
        The function <m>f</m> in Equation <xref ref="exp_iaz_P_z__Q_z_"/> is <m>f(z) = \frac{\exp (iz) z}{z^2+4}</m>,
        which has a simple pole at the point <m>2i</m> in the upper half-plane.
        Calculating the residue yields
        <me>
          \mathrm{Res}[f,2i] =\lim\limits_{z \to 2i}\frac{\exp(iz)z}{z+2i} = \frac{2ie^{-2}}{4i}=\frac{1}{2e^2}
        </me>.
        Using Equation <xref ref="PV__P_Q_sin_ax_"/> gives
        <me>
          \text{ P.V. }  \int_{-\infty}^{\infty}\frac{x\sin x}{x^2+4}\,dx = 2\pi \mathrm{Re}(\mathrm{Res}[f,2i]) = \frac{\pi}{e^2}
        </me>
      </p>
    </statement>
    <solution>
      <p>
        DD
      </p>
    </solution>
  </example>
  <example>
    <statement>
      <p>
        Evaluate P.V. <m>\int_{-\infty}^{\infty}\frac{\cos x\,dx}{x^4+4}</m>.
      </p>
      <p>
        The function <m>f</m> in Equation <xref ref="exp_iaz_P_z__Q_z_"/> is <m>f(z) = \frac{\exp (iz)}{z^4+4}</m>,
        which has simple poles at the points <m>z_1=1+i</m> and
        <m>z_2=-1+i</m> in the upper half-plane.
        We get the residues with the aid of L'H&#xf4;pital's rule:
        <md>
          <mrow>\mathrm{Res}[f, \, 1+i]  \amp = \lim_{z \to 1+i}\frac{(z-1-i) \exp (iz)}{z^4+4}</mrow>
          <mrow>\amp = \lim_{z \to 1+i}\frac{[1+i(z-1-i)]\exp (iz)}{4z^3}</mrow>
          <mrow>\amp = \frac{\exp (-1+i)}{4(1+i)^3}</mrow>
          <mrow>\amp = \frac{\sin 1-\cos 1-i(\cos 1+\sin 1)}{16e}</mrow>
        </md>.
      </p>
      <p>
        Similarly,
        <me>
          \mathrm{Res}[f, \, -1+i] = \frac{\cos 1 -\sin 1 -i(\cos 1+\sin 1)}{16e}
        </me>.
        Using Equation <xref ref="PV__P_Q_cos_ax_"/>, we get
        <md>
          <mrow>\int_{-\infty}^{\infty}\frac{\cos x}{x^4+4}\,dx \amp = -2\pi [\mathrm{Im}(\mathrm{Res}[f,1+i] ) + \mathrm{Im}(\mathrm{Res}[f,-1+i])]</mrow>
          <mrow>\amp = \frac{\pi (\cos 1+\sin 1)}{4e}</mrow>
        </md>.
      </p>
    </statement>
    <solution>
      <p>
        DD
      </p>
    </solution>
  </example>
  <p>
    We are almost ready to give the proof of <xref ref="PV_P_Q_sin__cos_thm">Theorem</xref>,
    but first we need one preliminary result.
  </p>
  <lemma xml:id="Jordan_s_Lemma">
    <title>Jordan's lemma</title>
    <statement>
      <p>
        Suppose that <m>P</m><nbsp/>and <m>Q</m><nbsp/>are polynomials of degree <m>m</m> and <m>n</m>,
        respectively, where <m>n \ge m+1</m>.
        If <m>C_R</m> is the upper semicircle <m>z=Re^{i\theta}</m>,
        for <m>0 \le \theta \le \pi</m>, then
        <me>
          \lim_{R \to \infty}\int_{c_{R}}\frac{\exp(iz)P(z)}{Q(z)}\,dz=0
        </me>.
      </p>
    </statement>
  </lemma>
  <proof>
    <p>
      From <m>n \ge m+1</m>, it follows that
      <m>|\frac{P(z)}{Q(z)}| \to 0</m> as <m>|z| \to \infty</m>.
      Therefore, for any <m>\varepsilon>0</m>,
      there exists <m>R_{\varepsilon}>0</m> such that
      <men xml:id="P_Q___e_Pi">
        |\frac{P(z)}{Q(z)}| \lt  \frac{\varepsilon}{\pi}
      </men>
      whenever <m>|z| \ge R_{\varepsilon}</m>.
      Using the ML inequality
      (<xref ref="ML_Inequality_Thm">Theorem</xref>)
      together with <xref ref="P_Q___e_Pi">Inequality</xref>, we get
      <men xml:id="Lemma_Integral">
        \left|\int_{C_R}\frac{\exp(iz)P(z)}{Q(z)}\,dz\right| \le \int_{C_R}\frac{\varepsilon}{\pi}|e^{iz}|\,|dz|
      </men>.
      provided <m>R\ge R_{\varepsilon}</m>.
      The parametrization of <m>C_R</m> leads to the equation
      <men xml:id="Lemma_Subs">
        |dz| = R\,d\theta,  \text{ and }   |e^{iz}|=e^{-y}=e^{-R\sin \theta}
      </men>.
    </p>
    <p>
      Using the trigonometric identity
      <m>\sin (\pi -\theta) = \sin \theta</m> and Equations <xref ref="Lemma_Subs"/>,
      we express the integral on the right side of <xref ref="Lemma_Integral">Inequality</xref> as
      <men xml:id="Lemma_Integral_2">
        \int_{C_R}\frac{\varepsilon}{\pi}|e^{iz}|\,|dz| = \frac{\varepsilon}{\pi}\int_0^{\pi}e^{-R\sin \theta}R\,d\theta = \frac{2\varepsilon}{\pi}\int_0^{\pi /2}e^{-R\sin \theta}R\,d\theta
      </men>.
    </p>
    <p>
      On the interval <m>0 \le \theta \le \pi /2</m> we can use the inequality
      <me>
        0 \le \frac{2\theta}{\pi}\le \sin \theta
      </me>.
      We combine this inequality with <xref ref="Lemma_Integral">Inequality</xref>
      and <xref ref="Lemma_Integral_2">Equation</xref> to conclude that,
      for <m>R \ge R_{\varepsilon}</m>,
      <md>
        <mrow>\left|\int_{C_R}\frac{\exp(iz)P(z)}{Q(z)}\,dz\right| \amp \le \frac{2\varepsilon}{\pi} \int_0^{\pi /2}e^{-\frac{2R\theta}{\pi}}R\,d\theta</mrow>
        <mrow>\amp = \left. -\varepsilon e^{-\frac{2R\theta}{\pi}}\right|_{\theta=0}^{\theta = \pi /2}</mrow>
        <mrow>\amp = \varepsilon (1-e^{-R})</mrow>
        <mrow>\amp \lt  \varepsilon</mrow>
      </md>.
    </p>
    <p>
      Because <m>\varepsilon >0</m> is arbitrary,
      the proof of Jordan's lemma is complete.
    </p>
  </proof>
  <p>
    We now turn to the proof of our main Theorem.
  </p>
  <proof>
    <p>
      Let <m>C</m> be the contour that consists of the segment
      <m>-R \le x \le R</m> of the real axis together with the upper semicircle <m>C_R</m><nbsp/>parametrized by <m>z=Re^{i\theta}</m>,
      for <m>0 \le \theta \le \pi</m>.
      Using properties of integrals, we have
      <me>
        \int_{-R}^{R}\frac{\exp(i\alpha x)P(x)}{Q(x)}\,dx = \int_{C}\frac{\exp(i\alpha z)P(z)}{Q(z)}\,dz - \int_{C_R}\frac{\exp(i\alpha z)P(z)}{Q(z)}\,dz
      </me>.
    </p>
    <p>
      If <m>R</m> is sufficiently large,
      all the poles <m>z_1, \, z_2, \, \ldots, \, z_k</m> of <m>f</m> will lie inside <m>C</m>,
      and we can use the residue theorem to obtain
      <men xml:id="Eq_8_12">
        \int_{-R}^{R} \frac{\exp (i\alpha x)P(x)}{Q(x)}\,dx = 2 \pi i\sum_{j=1}^k\mathrm{Res}[f,z_j] - \int_{C_R}\frac{\exp(i\alpha z)P(z)}{Q(z)}\,dz
      </men>.
    </p>
    <p>
      Since <m>\alpha</m> is a positive real number,
      the change of variables <m>\zeta=\alpha z</m> shows that the conclusion of Jordan's lemma holds for the integrand <m>\frac{\exp(i\alpha z)P(z)}{Q(z)}</m>.
      Hence we let <m>R \to \infty</m> in Equation <xref ref="Eq_8_12"/> to obtain
      <md>
        <mrow>\text{ P.V. }  \int_{-\infty}^{\infty}\frac{[\cos(\alpha x)+i\sin(\alpha x)]P(x)}{Q(x)}\,dx \amp = 2\pi i\sum_{j=1}^k\mathrm{Res}[f,z_j]</mrow>
        <mrow>\amp = -2\pi \sum\limits_{j=1}^k\mathrm{Im}(\mathrm{Res}[f,z_j])</mrow>
        <mrow>\amp + 2\pi i\sum\limits_{j=1}^k\mathrm{Re}(\mathrm{Res}[f,z_j])</mrow>
      </md>.
    </p>
    <p>
      Equating the real and imaginary parts of this equation gives us Equations <xref ref="PV__P_Q_cos_ax_"/> and <xref ref="PV__P_Q_sin_ax_"/>, which completes the proof.
    </p>
  </proof>
  <exercises xml:id="exercises_improper-trig-integrals">
    <title>Exercises</title>
    <p>
      Use residues to find the Cauchy principal value of the following:
    </p>
    <exercise xml:id="x8_4_1">
      <statement>
        <p>
          <m>\int_{-\infty}^{\infty}\frac{\cos x}{x^2+9}\,dx, \text{ and } \int_{-\infty}^{\infty}\frac{\sin x}{x^2+9}\,dx</m>.
        </p>
      </statement>
      <solution>
        <p>
          <m>\int_{-\infty}^{\infty}\frac{\cos x}{x^2+9}\,dx = \frac{\pi}{3e^3}</m>,
          and <m>\int_{-\infty}^{\infty}\frac{\sin x}{x^2+9}\,dx = 0</m>.
          DD
        </p>
      </solution>
    </exercise>
    <exercise xml:id="x8_4_2">
      <statement>
        <p>
          <m>\int_{-\infty}^{\infty}\frac{x\cos x}{x^2+9}\,dx, \text{ and } \int_{-\infty}^{\infty}\frac{x\sin x}{x^2+9}\,dx</m>.
        </p>
      </statement>
    </exercise>
    <exercise xml:id="x8_4_3">
      <statement>
        <p>
          <m>\int_{-\infty}^{\infty}\frac{x\sin x}{(x^2+4)^2}\,dx</m>.
        </p>
      </statement>
      <solution>
        <p>
          <m>\frac{\pi}{4e^2}</m>.
          DD
        </p>
      </solution>
    </exercise>
    <exercise xml:id="x8_4_4">
      <statement>
        <p>
          <m>\int_{-\infty}^{\infty}\frac{\cos x}{(x^2+4)^2}\,dx</m>.
        </p>
      </statement>
    </exercise>
    <exercise xml:id="x8_4_5">
      <statement>
        <p>
          <m>\int_{-\infty}^{\infty}\frac{\cos x}{(x^2+4)(x^2+9)}\,dx</m>.
        </p>
      </statement>
      <solution>
        <p>
          <m>\frac{\pi}{5}(\frac{1}{2e^2}-\frac{1}{3e^3})</m>.
          DD
        </p>
      </solution>
    </exercise>
    <exercise xml:id="x8_4_6">
      <statement>
        <p>
          <m>\int_{-\infty}^{\infty}\frac{\cos x}{(x^2+1)(x^2+4)}\,dx</m>.
        </p>
      </statement>
    </exercise>
    <exercise xml:id="x8_4_7">
      <statement>
        <p>
          <m>\int_{-\infty}^{\infty}\frac{\cos x}{x^2-2x+5}\,dx</m>.
        </p>
      </statement>
      <solution>
        <p>
          <m>\frac{\pi \cos 1}{2e^2}</m>.
          DD
        </p>
      </solution>
    </exercise>
    <exercise xml:id="x8_4_8">
      <statement>
        <p>
          <m>\int_{-\infty}^{\infty}\frac{\cos x}{x^2-4x+5}\,dx</m>.
        </p>
      </statement>
    </exercise>
    <exercise xml:id="x8_4_9">
      <statement>
        <p>
          <m>\int_{-\infty}^{\infty}\frac{x\sin x}{x^4+4}\,dx</m>.
        </p>
      </statement>
      <solution>
        <p>
          <m>\frac{\pi \sin 1}{2e}</m>.
          DD
        </p>
      </solution>
    </exercise>
    <exercise xml:id="x8_4_10">
      <statement>
        <p>
          <m>\int_{-\infty}^{\infty}\frac{x^3\sin x}{x^4+4}\,dx</m>.
        </p>
      </statement>
    </exercise>
    <exercise xml:id="x8_4_11">
      <statement>
        <p>
          <m>\int_{-\infty}^{\infty}\frac{\cos 2x}{x^2+2x+2}\,dx</m>.
        </p>
      </statement>
      <solution>
        <p>
          <m>\frac{\pi \cos 2}{e^2}</m>.
          DD
        </p>
      </solution>
    </exercise>
    <exercise xml:id="x8_4_12">
      <statement>
        <p>
          <m>\int_{-\infty}^{\infty}\frac{x^3\sin 2x}{x^4+4}\,dx</m>.
        </p>
      </statement>
    </exercise>
    <exercise xml:id="x8_4_13">
      <statement>
        <p>
          Why do you need to use the exponential function when evaluating improper integrals involving the sine and cosine functions?
        </p>
      </statement>
      <solution>
        <p>
          The inequality <m>\left|\int_{C_{R}}\frac{\exp(iz)P(z)}{Q(z)}\,dz\right| \le \frac{2\varepsilon}{\pi}\int\nolimits_0^\frac{\pi}{2}e^{\frac{-2R\theta}{\pi}}R\,d\theta \lt \varepsilon</m> in Jordan's lemma would not be possible to get if we replaced
          <m>\exp(iz)</m> by either the complex sine or cosine.
          Explain!
          DD
        </p>
      </solution>
    </exercise>
  </exercises>
</section>