<section xml:id="sec_complex-integrals">
  <title>Complex Integrals</title>
  <p>
    We introduce the integral of a complex function by defining the integral of a complex-valued function of a <em>real</em> variable.
  </p>
  <definition>
    <title>Integral of $f(t)$</title>
    <statement>
      <p>
        Let <m>f(t)=u(t)+iv(t)</m>,
        where <m>u</m> and <m>v</m> are real-valued functions of the real variable <m>t</m> for <m>a \le t \le b</m>.
        Then
        <men xml:id="Integral_Def_1">
          \int_a^b f(t)\,dt=\int_a^b u(t)\, dt+i\int_a^b v(t)\, dt
        </men>.
      </p>
    </statement>
  </definition>
  <p>
    We generally evaluate integrals of this type by finding the antiderivatives of <m>u</m> and <m>v</m> and evaluating the definite integrals on the right side of Equation <xref ref="Integral_Def_1"/>.
    That is, if <m>U\,'(t)=u(t)</m>,
    and <m>V\,'(t)=v(t)</m>, for <m>a \le t \le b</m>, we have
    <men xml:id="Integral_Def_2">
      \int_a^b f(t)\,dt = \big[U(t) +iV(t)\big] \Big|_{t=a}^{t=b}=U(b)-U(a) +i\big[V(b) -V(a)\big]
    </men>.
  </p>
  <example>
    <statement>
      <p>
        Show that
        <me>
          \int_0^1(t-i)^3\,dt=-\frac{5}{4}
        </me>.
      </p>
      <p>
        We write the integrand in terms of its real and imaginary parts,
        <em>i.e.</em>, <m>f(t)=(t-i)^3=t^3-3t+i(-3t^2+1)</m>.
        Here, <m>u(t)=t^3-3t</m> and <m>v(t)=-3t^2+1</m>.
        The integrals of <m>u</m> and <m>v</m> are
        <me>
          \int_0^1(t^3-3t)\,dt=-\frac{5}{4},  \text{ and }   \int_0^1(-3t^2+1) \,dt=0
        </me>.
      </p>
      <p>
        Hence, by <xref ref="Integral_Def_1">Definition</xref>,
        <me>
          \int_0^1(t-i)^3\,dt = \int_0^1u(t)\,dt+i\int_0^1v(t)\,dt = -\frac{5}{4}
        </me>
      </p>
    </statement>
    <solution>
      <p>
      </p>
    </solution>
  </example>
  <example xml:id="Int_ex">
    <statement>
      <p>
        Show that
        <me>
          \int_0^{\frac{\pi}{2}}\exp(t+it)\,dt = \frac{1}{2} (e^{\frac{\pi}{2}}-1) + \frac{i}{2}(e^{\frac{\pi}{2}}+1)
        </me>.
      </p>
      <p>
        We use the method suggested by <xref ref="Integral_Def_1">Definitions</xref>
        and <xref ref="Integral_Def_2"></xref>.
        <md>
          <mrow>\int_0^{\frac{\pi}{2}}\exp (t+it)\,dt \amp = \int_0^{\frac{\pi}{2}}e^te^{it}dt</mrow>
          <mrow>\amp = \int_0^{\frac{\pi}{2}}e^t(\cos t+i\sin t \,dt</mrow>
          <mrow>\amp = \int_0^{\frac{\pi}{2}}e^t\cos t \, dt + i\int_0^{\frac{\pi}{2}}e^t\sin t \,dt</mrow>
        </md>.
      </p>
      <p>
        We can evaluate each of the integrals via integration by parts.
        For example,
        <md>
          <mrow>\int_0^{\frac{\pi}{2}}\underset{u}{\underbrace{e^t}} \; \underset{dv}{\underbrace{\cos t\,dt}} \amp = (\underset{u}{\underbrace{e^t}} \; \underset{v}{\underbrace{\sin t}}) \Big|_{t=0}^{t=\frac{\pi}{2}} -\int_0^{\frac{\pi}{2}}\underset{v}{\underbrace{\sin t}} \; \underset{du}{\underbrace{e^tdt}}</mrow>
          <mrow>\amp = (e^{\frac{\pi}{2}}\sin \frac{\pi}{2}-e^0\sin 0) -\int_0^{\frac{\pi}{2}}\underset{u}{\underbrace{e^t}} \; \underset{dv}{\underbrace{\sin t \,dt}}</mrow>
          <mrow>\amp = e^{\frac{\pi}{2}}-\int_0^{\frac{\pi}{2}}\underset{u}{\underbrace{e^t}} \; \underset{dv}{\underbrace{\sin t \,dt}}</mrow>
          <mrow>\amp = e^{\frac{\pi}{2}} - (\underset{u}{\underbrace{e^t}} \; [\underset{v}{\underbrace{-\cos t}}] ) \Big|_{t=0}^{t=\frac{\pi}{2}} +\int_0^{\frac{\pi}{2}}\underset{v}{\underbrace{-\cos t}} \; \underset{du}{\underbrace{e^t\,dt}}</mrow>
          <mrow>\amp = e^{\frac{\pi}{2}}-1-\int_0^{\frac{\pi}{2}}e^t\cos t\,dt</mrow>
        </md>.
      </p>
      <p>
        Adding <m>\int_0^{\frac{\pi}{2}}e^t\cos t\,dt</m> to both sides of this equation and then dividing by 2 gives <m>\int_0^{\frac{\pi}{2}}e^t\cos t)\,dt=\frac{1}{2}(e^{\frac{\pi}{2}}-1)</m>.
        A similar computation procedure yields <m>i\int_0^{\frac{\pi}{2}}e^t\sin t\,dt=\frac{i}{2}(e^{\frac{\pi}{2}}+1)</m>.
        Therefore,
        <me>
          \int_0^{\frac{\pi}{2}}\exp (t+it)\,dt=\frac{1}{2}(e^{\frac{\pi}{2}}-1) + \frac{i}{2}(e^{\frac{\pi}{2}}+1)
        </me>
      </p>
    </statement>
    <solution>
      <p>
      </p>
    </solution>
  </example>
  <p>
    Complex integrals have properties that are similar to those of real integrals.
    We now trace through several commonalities.
    Let <m>f(t)=u(t)+iv(t)</m> and
    <m>g(t)=p(t)+iq(t)</m> be continuous on <m>a \le t \le b</m>.
    <ul>
      <li>
        <p>
          Using <xref ref="Integral_Def_1">Definition</xref>,
          we can easily show that the integral of their sum is the sum of their integrals, that is
          <men xml:id="Int_Prop_1">
            \int_a^b[f(t)+g(t)]\,dt = \int_a^bf(t)\,dt + \int_a^b g(t)\,dt
          </men>.
        </p>
      </li>
      <li>
        <p>
          If we divide the interval <m>a \le t \le b</m> into <m>a \le t \le c</m> and
          <m>c \le t \le b</m> and integrate <m>f(t)</m> over these subintervals by using <xref ref="Integral_Def_1">Definition</xref>,
          then we get
          <men xml:id="Int_Prop_2">
            \int_a^bf(t)\,dt=\int_{a}^{c}f(t)\,dt+\int_c^{b}f(t)\,dt
          </men>.
        </p>
      </li>
      <li>
        <p>
          Similarly, if <m>c+id</m> denotes a complex constant, then
          <men xml:id="Int_Prop_3">
            \int_a^b(c+id) f(t)\,dt=(c+id) \int_a^bf(t)\,dt
          </men>.
        </p>
      </li>
      <li>
        <p>
          If the limits of integration are reversed, then
          <men xml:id="Int_Prop_4">
            \int_a^bf(t)\,dt=-\int_{b}^{a}f(t)\,dt
          </men>.
        </p>
      </li>
      <li>
        <p>
          The integral of the product <m>fg</m> becomes
          <md>
            <mrow>\int_a^bf(t) g(t)\,dt \amp = \int_a^b \big[u(t) p(t) -v(t) q(t)\big] \, dt</mrow>
            <mrow xml:id="Int_Prop_5" number="yes">\amp + i\int_a^b \big[u(t)q(t) + v(t)p(t)\big] \, dt</mrow>
          </md>.
        </p>
      </li>
    </ul>
  </p>
  <example>
    <statement>
      <p>
        Let us verify Property <xref ref="Int_Prop_3"/>.
        We start by writing
        <me>
          (c+id) f(t)= (c+id)\big(u(t) + iv(t)\big)= cu(t) -dv(t) +i \big[cv(t) +du(t)\big]
        </me>.
        Using <xref ref="Integral_Def_1">Definition</xref>,
        we write the left side of <xref ref="Int_Prop_3">Equation</xref> as
        <me>
          c\int_a^bu(t)\,dt-d\int_a^bv(t)\,dt + ic\int_a^bv(t) \, dt + id\int_a^bu(t)\,dt
        </me>.
        which is equivalent to
        <me>
          (c+id) \left[ \int_a^bu(t)\,dt + i\int_a^bv(t)\,dt\right]
        </me>
      </p>
    </statement>
  </example>
  <p>
    It is worthwhile to point out the similarity between Equation <xref ref="Integral_Def_2"/> and its counterpart in calculus.
    Suppose that <m>U</m> and <m>V</m> are differentiable on
    <m>a\lt t\lt b</m> and <m>F(t)=U(t)+iV(t)</m>.
    Since <m>F\,'(t)=U\,'(t) +iV\,'(t) =u(t) +iv(t)=f(t)</m>, Equation <xref ref="Integral_Def_2"/> takes on the familiar form
    <men xml:id="Integral_Def_4">
      \int_a^bf(t)\,dt =  F(t) \Big|_{t=a}^{t=b}=F(b) -F(a)
    </men>.
    where <m>F\,'(t)=f(t)</m>.
    We can view Equation <xref ref="Integral_Def_4"/> as an extension of the fundamental theorem of calculus.
    In <xref ref="sec_integral-representations">Section</xref>
    we show how to generalize this extension to analytic functions of a complex variable.
    For now, we simply note an important case of Equation <xref ref="Integral_Def_4"/>:
    <men xml:id="Int_Prop_6">
      \int_a^bf\,'(t)\,dt=f(b)-f(a)
    </men>.
  </p>
  <example xml:id="ex_6_4">
    <statement>
      <p>
        Use Equation <xref ref="Integral_Def_4"/> to show that
        <me>
          \int_0^{\frac{\pi}{2}}\exp(t+it)\,dt=\frac{1}{2} (e^{\frac{\pi}{2}}-1) + \frac{i}{2}(e^{\frac{\pi}{2}}+1)
        </me>
      </p>
    </statement>
    <solution>
      <p>
        We seek a function <m>F</m> with the property that <m>F\,'(t)= \exp(t+it)</m>.
        We note that <m>F(t)=\frac{1}{1+i} e^{t(1+i)}</m> satisfies this requirement, so
        <md>
          <mrow>\int_0^{\frac{\pi}{2}}\exp (t+it)\,dt \amp = \frac{ 1}{1+i}e^{t(1+i)}\Big|_{t=0}^{t=\frac{\pi}{2}}=\frac{1}{ 1+i}(ie^{\frac{\pi}{2}}-1)</mrow>
          <mrow>\amp = \frac{1}{2}(1-i) (ie^{\frac{\pi}{2}}-1)</mrow>
          <mrow>\amp  \frac{1}{2}(e^{\frac{\pi}{2}}-1) +\frac{i}{2}(e^{\frac{ \pi}{2}}+1)</mrow>
        </md>,
        which is the same result we obtained in <xref ref="Int_ex">Example</xref>,
        but with a lot less work!
      </p>
    </solution>
  </example>
  <remark xml:id="advantage">
    <p>
      <xref ref="ex_6_4">Example</xref>
      illustrates the potential computational advantage we have when we lift our sights to the complex domain.
      Using ordinary Calculus techniques to evaluate <m>\int_0^{\frac{\pi}{2}}e^t\cos t)\,dt</m>,
      for example,
      would require a lengthy integration by parts procedure.
      When we recognize this expression as the real part of <m>\int_0^{\frac{\pi}{2}}\exp (t+it)\,dt</m>,
      however, the solution comes quickly.
      This is just one of the many reasons why good physicists and engineers,
      in addition to mathematicians,
      benefit from a thorough working knowledge of complex analysis.
    </p>
  </remark>
  <exercises xml:id="exercises_complex-integrals">
    <title>Exercises</title>
    <exercise xml:id="x6_1_1">
      <introduction>
        <p>
          Use Equations <xref ref="Integral_Def_1"/> and <xref ref="Integral_Def_2"/> to find
        </p>
      </introduction>
      <task>
        <statement>
          <p>
            <m>\int_0^1(3t-i)^2dt</m>.
          </p>
        </statement>
        <solution>
          <p>
            <m>2-3i</m>.
          </p>
        </solution>
      </task>
      <task>
        <p>
          <m>\int_0^1(t+2i)^3dt</m>.
        </p>
      </task>
      <task>
        <statement>
          <p>
            <m>\int_0^{\frac{\pi}{2}}\cosh (it)\,dt</m>.
          </p>
        </statement>
        <solution>
          <p>
            <m>1</m>.
          </p>
        </solution>
      </task>
      <task>
        <p>
          <m>\int_0^2\frac{t}{t+i}dt</m>.
        </p>
      </task>
      <task>
        <statement>
          <p>
            <m>\int_0^{\frac{\pi}{4}}t\exp (it)\,dt</m>.
          </p>
        </statement>
        <solution>
          <p>
            <m>\frac{\sqrt{2}\pi}{8} + \frac{\sqrt{2}}{2} - 1 + i(\frac{\sqrt{2}}{2} - \frac{\sqrt{2}\pi}{8})</m>.
          </p>
        </solution>
      </task>
    </exercise>
    <exercise xml:id="x6_1_2">
      <statement>
        <p>
          Let <m>m</m> and <m>n</m> be integers.
          Show that
          <me>
            \int_0^{2\pi}e^{imt}e^{-int}\,dt = \begin{cases}\; 0, \amp  \text{ when } \; m \ne n;\\ 2\pi, \amp  \text{ when } \; m = n. \end{cases}
          </me>
        </p>
      </statement>
    </exercise>
    <exercise xml:id="x6_1_3">
      <statement>
        <p>
          Show that <m>\int_0^{\infty}e^{-zt}dt=\frac{1}{z}</m> provided <m>\mathrm{Re}(z) >0</m>.
        </p>
      </statement>
      <solution>
        <p>
          Using Equation <xref ref="Integral_Def_4"/> we get <m>\int_0^{\infty}e^{-zt}\,dt = \lim\limits_{T \to \infty}\int_0^{T}e^{-zt}\,dt = \lim\limits_{T \to \infty}(-\frac{1}{z}e^{-zT} + \frac{1}{z}e^{-z(0)}) = \frac{1}{z} + \lim\limits_{T \to \infty}(-\frac{1}{z}e^{-zT})</m>.
          Show that <m>\mathrm{Re}(z)>0</m> implies this last limit equals zero.
        </p>
      </solution>
    </exercise>
    <exercise xml:id="x6_1_4">
      <introduction>
        <p>
          Establish the following identities .
        </p>
      </introduction>
      <task>
        <p>
          Identity <xref ref="Int_Prop_1"/>.
        </p>
      </task>
      <task>
        <p>
          Identity <xref ref="Int_Prop_2"/>.
        </p>
      </task>
      <task>
        <p>
          Identity <xref ref="Int_Prop_4"/>.
        </p>
      </task>
      <task>
        <p>
          Identity <xref ref="Int_Prop_5"/>.
        </p>
      </task>
    </exercise>
    <exercise>
      <statement>
        <p>
          Let <m>f(t)=u(t) +iv(t)</m>, where <m>u</m> and <m>v</m> are differentiable.
          Show that
          <men xml:id="x6_1_5">
            \int_a^bf(t) f\,'(t)\,dt=\frac{1}{2}[f(b)]^2-\frac{1}{2}\left[ f(a) \right] ^2
          </men>
        </p>
      </statement>
      <solution>
        <p>
          This follows from Equation <xref ref="Integral_Def_4"/>,
          and the fact that if <m>u</m> and <m>v</m> are differentiable,
          then <m>f</m> is differentiable,
          and <m>\frac{d}{dt}\left[\frac{1}{2}\big(f(t)\big)^2\right] = f(t)f\,'(t)</m>.
        </p>
      </solution>
    </exercise>
    <exercise>
      <statement>
        <p>
          Use integration by parts to verify that <m>i\int_0^{\frac{\pi}{2}}e^t\sin t)\,dt=\frac{i}{2}(e^{\frac{\pi}{2}}+1)</m>.\label {6.1.6}
        </p>
      </statement>
    </exercise>
  </exercises>
</section>