<section xml:id="sec_fourier-series">
  <title>Fourier Series</title>
  <introduction>
    <p>
      In this chapter we show how Fourier series, the Fourier transform,
      and the Laplace transform are related to the study of complex analysis.
      We develop the Fourier series representation of a real-valued function <m>U(t)</m> of the real variable <m>t</m>.
      Complex Fourier series and Fourier transforms are then discussed.
      Finally, we develop the Laplace transform and the complex variable technique for finding its inverse.
      This chapter focuses on applying these ideas to solving problems involving real-valued functions,
      so many of the theorems throughout are stated without proof.
    </p>
    <p>
      Let <m>U(t)</m> be a real-valued function that is periodic with period <m>2\pi</m>, that is,
      <me>
        U(t+2\pi)=U(t)  \text{ for all } t
      </me>.
      One such function is <m>s= U(t) = \sin(t-\frac{\pi}{2}) + 0.7\cos(2t-\pi -\frac{1}{4}) +1.7</m>,
      and its graph is obtained by repeating the portion of the graph in any interval of length <m>2\pi</m>,
      as shown in <xref ref="fig_ch-11-01">Figure</xref>.
    </p>
    <figure xml:id="fig_ch-11-01">
      <caption>A function <m>U</m> with period <m>2\pi</m></caption>
      <image width="73%" source="figs/ch-11/ch-11-fig-01.png"/>
    </figure>
    <p>
      Familiar examples of real functions that have period <m>2\pi</m> are <m>\sin nt</m> and <m>\cos nt</m>,
      where <m>n</m> is an integer.
      This raises the question whether any periodic function can be represented by a sum of terms involving
      <m>a_n\cos nt</m> and <m>b_n\sin nt</m>,
      where <m>a_n</m> and <m>b_n</m> are real constants.
      As we shall soon see, the answer to this question is often yes.
    </p>
    <definition>
      <title>Piecewise Continuous</title>
      <statement>
        <p>
          The function <m>U</m> is piecewise continuous on the closed interval <m>[a,b]</m> if there exists values <m>t_0,t_1,\ldots,t_n</m> with
          <m>a = t_0\lt t_1\lt \cdots\lt t_n=b</m> such that <m>U</m> is continuous in each of the open intervals
          <m>t_{k-1}\lt t\lt t_k(k=1,2,...n)</m> and has left- and right-hand limits at the values <m>t_k</m> for <m>k=0,1,\ldots, n</m>.
        </p>
      </statement>
    </definition>
    <p>
      We use the symbols <m>U(a^-)</m> and <m>U(a^+)</m> for the left- and right-hand limits,
      respectively,
      of a function <m>U(t)</m> as <m>t</m> approaches the point <m>a</m>.
      The graph of a piecewise continuous function is illustrated in <xref ref="fig_ch-11-02">Figure</xref>.
      <me>
        U(t) =\left\{
        <tabular>
          <row>
            <cell>\(\frac{2}{3}(t-\frac{1}{2})^2+\frac{1}{4}\)</cell>
            <cell>\(\text{ when }  1 \le t\lt 2,\)</cell>
          </row>
          <row>
            <cell>\(\frac{5}{2}-(t-2)^2\)</cell>
            <cell>\(\text{ when }  2\lt t\lt 3,\)</cell>
          </row>
          <row>
            <cell>\(1+\frac{t-3}{4}\)</cell>
            <cell>\(\text{ when }  3\lt t\lt 4,\)</cell>
          </row>
          <row>
            <cell>\(\frac{6}{5}-(t-5)^3\)</cell>
            <cell>\(\text{ when }  4\lt t \le 6\).</cell>
          </row>
        </tabular>
        \right.
      </me>
    </p>
    <figure xml:id="fig_ch-11-02">
      <caption>A piecewise continuous function <m>U</m> over the interval <m>[1,6]</m></caption>
      <image width="73%" source="figs/ch-11/ch-11-fig-02.png"/>
    </figure>
    <p>
      The left- and right-hand limits at <m>t_0=2</m>,
      <m>t_1=3</m>, and <m>t_2=4</m> are easy to determine:
      <me>
        <tabular>
          <row>
            <cell>At \(t=2\), \ \  \(U(2^-) = \frac{7}{4}\) \ \  and \ \  \(U(2^+) = \frac{5}{2}\).</cell>
          </row>
          <row>
            <cell>At \(t=3\), \ \  \(U(3^-) = \frac{3}{2}\) \ \  and \ \  \(U(3^+) = 1\).</cell>
          </row>
          <row>
            <cell>At \(t=4\), \ \  \(U(4^-) = \frac{5}{4}\) \ \  and \ \  \(U(4^+) = \frac{11}{5}\).</cell>
          </row>
        </tabular>
      </me>
    </p>
    <definition>
      <title>Fourier Series</title>
      <statement>
        <p>
          If <m>U(t)</m> is periodic with period <m>2\pi</m> and is piecewise continuous on
          <m>[-\pi ,\pi]</m> then the Fourier series <m>S(t)</m> for <m>U(t)</m> is
          <men xml:id="FourierSdef">
            S(t) = \frac{a_0}{2} + \sum_{n=1}^{\infty}(a_n\cos nt + b_n\sin jt)
          </men>,
          where the coefficients <m>a_n</m> and <m>b_n</m> are given by the so-called Euler's Formulas:
          <men xml:id="FourierCoeffA">
            a_n = \frac{1}{\pi}\int_{-\pi}^{\pi}U(t)\cos nt\,dt  \text{ for }   n=0,1, \ldots
          </men>
          and
          <men xml:id="FourierCoeffB">
            b_n = \frac{1}{\pi}\int_{-\pi}^{\pi}U(t) \sin nt\,dt  \text{ for }   n=1,2, \ldots
          </men>
        </p>
      </statement>
    </definition>
    <p>
      The factor <m>\frac{1}{2}</m> in the constant term
      <m>\frac{a_0}{2}</m> on the right side of Equation <xref ref="FourierSdef"/> has been introduced for convenience so that <m>a_0</m> could be obtained from the general formula in Equation <xref ref="FourierCoeffA"/> by setting <m>j=0</m>.
      The reasons for this will be explained shortly.
      The next result discusses convergence of the Fourier series.
    </p>
    <theorem xml:id="thm_fourier-expansion">
      <title>Fourier Expansion</title>
      <statement>
        <p>
          Assume that <m>S(t)</m> is the Fourier series for <m>U(t)</m>.
          If <m>U\,'(t)</m> is piecewise continuous on <m>[-\pi ,\pi]</m>,
          then <m>S(t)</m> is convergent for all
          <m>t \in [-\pi,\pi ]</m> where <m>U(t)</m> is continuous.
          If <m>t=a</m> is a point of discontinuity of <m>U</m>, then
          <me>
            S(a) = \frac{U(a^-) +U(a^+)}{2}
          </me>,
          where <m>U(a^-)</m> and <m>U(a^+)</m> denote the left- and right-hand limits,
          respectively.
          With this understanding, we have the Fourier expansion:
          <men xml:id="FourierExpansion">
            U(t) = \frac{a_0}{2}+\sum\limits_{n=1}^{\infty}(a_n\cos nt+b_n\sin nt)
          </men>.
        </p>
      </statement>
    </theorem>
    <example xml:id="ex_11_1">
      <statement>
        <p>
          Show that the function <m>U(t) =\frac{t}{2}</m> for <m>t \in (-\pi ,\pi)</m>,
          extended periodically by the equation <m>U(t+2\pi)=U(t)</m>,
          has the Fourier series expansion
          <me>
            U(t) = \sum_{n=1}^{\infty}\frac{(-1)^{n+1}}{n}\sin nt
          </me>
        </p>
      </statement>
      <solution>
        <p>
          Using Euler's <xref ref="FourierCoeffA">Formulas</xref>
          and integration by parts, we obtain
          <me>
            a_n=\frac{1}{\pi}\int_{-\pi}^{\pi}\frac{t}{2}\cos nt\,dt = \left.\left(\frac{t\sin nt }{2\pi n} + \frac{\cos nt}{2\pi n^2}\right)\right|_{-\pi}^{\pi} = 0  \text{ for }   n=1,2,\ldots
          </me>,
          and then using Formula <xref ref="FourierCoeffB"/> we get
          <md>
            <mrow>b_n \amp = \frac{1}{\pi}\int_{-\pi}^{\pi}\frac{t}{2}\sin nt\,dt = \left.\left(\frac{ -t\cos nt}{2\pi n}+\frac{\sin nt}{2\pi n^2}\right)\right|_{-\pi}^{\pi}</mrow>
            <mrow>\amp =\frac{-\cos n\pi}{n}=\frac{(-1)^{n+1}}{n}  \text{ for }   n=1,2,\ldots \, </mrow>
          </md>.
        </p>
        <p>
          The coefficient <m>a_0</m> is computed by the calculation
          <me>
            a_0=\frac{1}{\pi}\int_{-\pi}^{\pi}\frac{t}{2}\,dt = \frac{t^2}{4\pi}\bigg|_{-\pi}^{\pi}=0
          </me>.
        </p>
        <p>
          Substituting the coefficients <m>a_j</m> and <m>b_j</m> in Equation <xref ref="FourierSdef"/> produces the required solution.
          The graphs of <m>U(t)</m> and the first three partial sums <m>S_1(t) = \sin t, \, S_2(t) = \sin t-\frac{1}{2}\sin 2t</m>,
          and <m>S_3(t) = \sin t-\frac{1}{2}\sin 2t + \frac{1}{3}\sin 3t</m> are shown in <xref ref="fig_ch-11-03">Figure</xref>.
        </p>
      </solution>
    </example>
    <figure xml:id="fig_ch-11-03">
      <caption><m>U(t) =\frac{t}{2}</m>, and approximations <m>S_1(t), \  S_2(t)</m>, and <m>S_3(t)</m></caption>
      <image width="73%" source="figs/ch-11/ch-11-fig-03.png"/>
    </figure>
    <p>
      We now state some general properties of Fourier series that are useful for calculating the coefficients.
      The proofs are left for the reader.
    </p>
    <theorem>
      <statement>
        <p>
          If <m>U(t)</m> and <m>V(t)</m> have Fourier series representations,
          then their sum <m>W(t)=U(t)+V(t)</m> has a Fourier series representation,
          and the Fourier coefficients of <m>W</m> are obtained by adding the corresponding coefficients of <m>U</m> and <m>V</m>.
        </p>
      </statement>
    </theorem>
    <theorem xml:id="thm_fourier-cosine">
      <title>Fourier Cosine Series</title>
      <statement>
        <p>
          Assume that <m>U(x)</m> is an even function.
          If <m>U(t)</m> has period <m>2\pi</m>,
          and <m>U(t)</m> and <m>U\,'(t)</m> are piecewise continuous,
          then the Fourier series for <m>U(t)</m> involves only the cosine terms,
          <em>i.e.</em>,
          <m>b_n=0</m>  for all <m>n</m>:
          <me>
            U(t) = \frac{a_0}{2}+\sum\limits_{n=1}^{\infty}a_n\cos nt
          </me>,
          where
          <me>
            a_n = \frac{2}{\pi}\int_0^{\pi}U(t)\cos nt\,dt,  \text{ for }   n=0,1,\ldots \
          </me>,
        </p>
      </statement>
    </theorem>
    <theorem>
      <title>Fourier Sine Series</title>
      <statement>
        <p>
          Assume that <m>U(t)</m> is an odd function.
          If <m>U(t)</m> has period <m>2\pi</m> and if <m>U(t)</m> and <m>U\,'(x)</m> are piecewise continuous,
          then the Fourier series for <m>U(t)</m> involves only sine terms,
          <em>i.e.</em>, <m>a_n=0</m> for all <m>n</m>:
          <me>
            U(t) = \sum_{n=1}^{\infty}b_n \sin nt
          </me>,
          where
          <me>
            b_n = \frac{2}{\pi}\int_0^{\pi}U(t) \sin nt\,dt  \text{ for }   n=1,2, \ldots \
          </me>,
        </p>
      </statement>
    </theorem>
    <theorem>
      <title>Termwise Integration</title>
      <statement>
        <p>
          If <m>U(t)</m> has a Fourier series representation given in <xref ref="FourierExpansion">Equation</xref>,
          then the integral of <m>U(t)</m> has a Fourier series representation which can be obtained by termwise integration of the Fourier Series of <m>U(t)</m>, that is,
          <me>
            \int_0^tU(\tau) = \sum_{n=1}^{\infty}\left(\frac{a_n+a_0(-1)^{n+1}}{n}\sin nt-\frac{b_n}{n}\cos nt\right)
          </me>,
          where we have used the expansion
          <m>a_0(\frac{t}{2}) = \sum\limits_{n=1}^{\infty}\frac{a_0(-1)^{n+1}}{n}\sin nt</m> from <xref ref="ex_11_1">Example</xref>.
        </p>
      </statement>
    </theorem>
    <theorem>
      <title>Termwise Differentiation</title>
      <statement>
        <p>
          If <m>U\,'(t)</m><em>has a Fourier series representation,
          and <m>U(t)</m> is given by Equation <xref ref="FourierExpansion"/>, then</em>
          <me>
            U\,'(t) =\sum\limits_{n=1}^{\infty}(nb_n\cos nt-na_n\sin jn)
          </me>
        </p>
      </statement>
    </theorem>
    <example>
      <statement>
        <p>
          Show that the function <m>U(t) = |t|</m> for <m>t \in (-\pi ,\pi)</m>,
          extended periodically the equation <m>U(t+2\pi) =U(t)</m>,
          has the Fourier series representation
          <me>
            U(t) = |t| = \frac{\pi}{2}-\frac{4}{\pi}\sum_{n=1}^{\infty}\frac{1}{(2n-1)^2}\cos[(2n-1)t]
          </me>
        </p>
      </statement>
      <solution>
        <p>
          The function <m>U(t)</m> is an even function,
          hence we can use <xref ref="thm_fourier-cosine">Theorem</xref>
          to conclude that <m>b_n=0</m> for all <m>n</m>, and
          <md>
            <mrow>a_n \amp = \frac{2}{\pi}\int_0^{\pi}t\cos nt\,dt=\left.\left(\frac{2t\sin nt}{\pi n}+ \frac{2\cos nt}{\pi n^2}\right)\right|_0^{\pi}</mrow>
            <mrow>\amp = \frac{2\cos n\pi -2}{\pi n^2}=\frac{2(-1)^n-2}{\pi n^2}  \text{ for }   n=1,2, \ldots \,</mrow>
          </md>.
        </p>
        <p>
          The coefficient <m>a_0</m> is computed by the calculation:
          <me>
            a_0=\frac{2}{\pi}\int_0^{\pi}t\,dt=\left.\frac{t^2}{\pi}\right|_0^{\pi}=\pi
          </me>.
          Using the <m>a_n</m> and <xref ref="thm_fourier-cosine">Theorem</xref>
          produces the required solution.
        </p>
      </solution>
    </example>
  </introduction>
  <subsection xml:id="subsec_euler-formula">
    <title>Proof of Euler's Formulas</title>
    <p>
      The following intuitive proof will justify the Euler formulas given in Equations <xref ref="FourierCoeffA"/> and <xref ref="FourierCoeffB"/> To determine <m>a_0</m> we integrate both <m>U(t)</m> and the Fourier series representation in Equation <xref ref="FourierSdef"/> from <m>-\pi</m> to <m>\pi</m>,
      which results in
      <me>
        \int_{-\pi}^{\pi}U(t)\,dt = \int_{-\pi}^{\pi}\left[\frac{a_0}{2} + \sum_{n=1}^{\infty}(a_n\cos nt+b_n\sin nt)\right]dt
      </me>.
      Next, we perform integration term by term, and we obtain
      <me>
        \int_{-\pi}^{\pi}U(t)\,dt = \frac{a_0}{2}\int_{-\pi}^{\pi}1\,dt + \sum_{n=1}^{\infty}a_n\int_{-\pi}^{\pi}\cos nt\,dt + \sum\limits_{n=1}^{\infty}b_n\int_{-\pi}^{\pi}\sin nt\,dt
      </me>.
      The value of the first integral on the right side of this equation is <m>2\pi</m> and all the other integrals are zero.
      Hence we obtain the desired formula for <m>a_0</m>:
      <me>
        a_0=\frac{1}{\pi}\int_{-\pi}^{\pi}U(t)\,dt
      </me>.
      To determine <m>a_m</m>,
      we let <m>m>1</m> denote a fixed integer and multiply both <m>U(t)</m> and the Fourier series representation in Equation <xref ref="FourierSdef"/> by the term <m>\cos mt</m>,
      and then we integrate and obtain
      <md>
        <mrow xml:id="CoeffA" number="yes">\int_{-\pi}^{\pi}U(t)\cos mt\,dt \amp = \frac{a_0}{2}\int_{-\pi}^{\pi}\cos mt\,dt</mrow>
        <mrow>\amp + \sum_{n=1}^{\infty}a_j\int_{-\pi}^{\pi}\cos mt\cos nt\,dt + \sum_{n=1}^{\infty}b_n\int_{-\pi}^{\pi}\cos mt\sin nt\,dt</mrow>
      </md>.
    </p>
    <p>
      The value of the first term on the right side of Equation <xref ref="CoeffA"/> is easily seen to be zero:
      <men xml:id="CoeffA0">
        \frac{a_0}{2}\int_{-\pi}^\pi\cos mt\,dt = \frac{a_0\sin mt}{2m}\bigg|_{-\pi}^\pi = 0
      </men>.
    </p>
    <p>
      The value of the term involving
      <m>\cos mt\cos jt</m> is found by using the trigonometric identity:
      <me>
        \cos mt\cos nt = \frac{1}{2} \Big(\cos [(m+n) t] +\cos [(m-n) t]\Big)
      </me>.
      Calculation reveals that if <m>m \ne n</m>
      (and <m>m>0</m>),
      then
      <md>
        <mrow xml:id="CoeffA1" number="yes">a_n\int_{-\pi}^{\pi}\cos mt\cos nt\,dt \amp = \frac{a_m}{2} \left[ \int_{-\pi}^{\pi}\cos[(m+n)t]\,dt\right. + \left.\int_{-\pi}^{\pi}\cos [(m-n) t] dt\right]</mrow>
        <mrow>\amp = 0</mrow>
      </md>.
    </p>
    <p>
      When <m>m=n</m>, the value of the integral becomes:
      <men xml:id="CoeffA2">
        a_m\int_{-\pi}^{\pi}\cos^2mt\,dt = \pi a_m
      </men>.
    </p>
    <p>
      The value of the term on the right side of Equation <xref ref="CoeffA"/> involving the integrand
      <m>\cos mt\sin nt</m> is found by using the trigonometric identity
      <me>
        \cos mt\sin nt=\frac{1}{2}\Big(\sin \big[(m+n)t\big] + \sin\big[(m-n)t\big]\Big)
      </me>,
      and for all values of <m>m</m> and <m>n</m>, we obtain
      <md>
        <mrow>b_n\int_{-\pi}^{\pi}\cos mt\sin nt\,dt \amp = \frac{b_m}{2}\left[\int_{-\pi}^\pi\sin[(m+n)t]\,dt\right.</mrow>
        <mrow xml:id="CoeffA3" number="yes">\amp + \left. \int_{-\pi}^\pi\sin[(m-n)t]\,dt\right]</mrow>
        <mrow>\amp = 0</mrow>
      </md>.
    </p>
    <p>
      Therefore, we can use the results of Equations <xref ref="CoeffA0"/><ndash/><xref ref="CoeffA3"/> in Equation <xref ref="CoeffA"/> to obtain
      <me>
        \int_{-\pi}^{\pi}U(t)\cos mt\,dt=\pi a_m  \text{ for }   m=0,1,2, \ldots
      </me>,
      and Equation <xref ref="FourierCoeffA"/> is established.
      We leave it as an exercise to establish Euler's <xref ref="FourierCoeffB">Formula</xref>
      for the coefficients <m>\left\{ b_n\right\}</m>.
      A complete discussion of the details of the proof of <xref ref="thm_fourier-expansion">Theorem</xref>
      can be found in some advanced texts.
      See for instance, John W. Dettman,
      <xref ref="ch_residue"/> in <em>Applied Complex Variables,</em>
      The Macmillan Company, New York, 1965.
    </p>
    <exercises xml:id="exercises_fourier-series">
      <title>Exercises</title>
      <task>
        <p>
          For Exercises 1<ndash/>2 and 6<ndash/>11,
          find the Fourier series representation.
        </p>
        <p>
          \begin{enumerate}
        </p>
      </task>
      <task>
        <p>
          <m>U(t) = \begin{cases}1 \;\;\, \text{ for } 0\lt t\lt \pi, \\ -1 \text{ for } -\pi \lt t\lt 0. \end{cases}</m> See <xref ref="fig_ch-11-04">Figure</xref>.
        </p>
        <p>
          \solution{ <m>U(t) =\frac{4}{\pi}\sum\limits_{n=1}^{\infty }\frac{1}{2n-1}\sin [(2n-1)t]</m>. }
        </p>
      </task>
      <task>
        <p>
          <m>V(t) = \begin{cases}\frac{\pi}{2}-t \text{ for } 0 \le t \le \pi . \\ \frac{\pi}{2}+t \text{ for } -\pi \lt t\lt 0. \end{cases}</m> See <xref ref="fig_ch-11-05">Figure</xref>.
        </p>
        <figure xml:id="fig_ch-11-04">
          <image width="73%" source="figs/ch-11/ch-11-fig-04.png"/>
        </figure>
        <figure xml:id="fig_ch-11-05">
          {0.5\linewidth}
          <image width="73%" source="figs/ch-11/ch-11-fig-05.png"/>
        </figure>
      </task>
      <task>
        <p>
          For Exercises 1 and 2, verify that
          <m>U(t) =-V'(t)</m> by termwise differentiation of the Fourier series representation for <m>V(t)</m>.
        </p>
        <p>
          \solution{ <m>V\,'(t)=\frac{4}{\pi}\sum\limits_{n=1}^{\infty }\frac{1}{(2n-1)^2}\frac{d}{dt}\cos[(2n-1)t] = -\frac{4}{\pi} \sum\limits_{n=1}^{\infty}\frac{1}{2n-1}\sin[(2n-1)t] = -U(t)</m>.
        </p>
      </task>
      <task>
        <p>
          For Exercise 1, set <m>t=\frac{\pi}{2}</m> and conclude that <m>\frac{\pi}{4}=\sum\limits_{j=1}^{\infty}\frac{(-1)^{j-1}}{2j-1}</m>.
        </p>
      </task>
      <task>
        <p>
          For Exercise 2, set <m>t=0</m> and conclude that <m>\frac{\pi^2}{8} = \sum\limits_{j=1}^{\infty}\frac{1}{(2j-1)^2}</m>.
        </p>
        <p>
          \solution{ <m>\frac{\pi }{2} = V(0) = \frac{4}{\pi}\sum\limits_{n=1}^{\infty} \frac{1}{(2n-1)^2}\cos(0)=\frac{4}{\pi }\sum\limits_{n=1}^{\infty}\frac{1}{(2n-1)^2}</m>.
          Now solve for <m>\sum\limits_{n=1}^{\infty}\frac{1}{(2n-1)^2}</m>. }
        </p>
      </task>
      <task>
        <p>
          <m>U(t) = \begin{cases}-1 \text{ for } \frac{\pi}{2} \lt t \lt \pi, \\ \;\;\, 1 \text{ for } -\frac{\pi}{2}\lt t \lt \frac{\pi}{2}, \\ -1 \text{ for } -\pi \lt t \lt -\frac{\pi}{2}. \end{cases}</m> See <xref ref="fig_ch-11-06">Figure</xref>.
        </p>
      </task>
      <task>
        <p>
          <m>U(t) = \begin{cases}\pi -t \text{ for } \frac{\pi}{2}\lt t\lt \pi, \\ t \text{ for } -\frac{\pi}{2}\lt t\lt \frac{\pi}{2}, \\ -\pi -t \text{ for } -\pi \lt t \lt -\frac{\pi}{2}. \end{cases}</m> See <xref ref="fig_ch-11-07">Figure</xref>.
        </p>
        <p>
          \solution{ <m>U(t)=\frac{4}{\pi}\sum\limits_{n=1}^{\infty}\frac{(-1)^{n-1}}{(2n-1)^2}\sin[(2n-1)t]</m>. }
        </p>
        <figure xml:id="fig_ch-11-06">
          <image width="73%" source="figs/ch-11/ch-11-fig-06.png"/>
        </figure>
        <figure xml:id="fig_ch-11-07">
          {0.5\linewidth}
          <image width="73%" source="figs/ch-11/ch-11-fig-07.png"/>
        </figure>
      </task>
      <task>
        <p>
          <m>U(t)</m>,
          as defined in <xref ref="fig_ch-11-08">Figure</xref>.
        </p>
      </task>
      <task>
        <p>
          <m>U(t) = \begin{cases}1 \;\;\, \text{ for } \frac{\pi}{2} \lt t \lt \pi, \\ 0 \;\;\, \text{ for } -\frac{\pi}{2}\lt t\lt \frac{\pi}{2}, \\ -1 \text{ for } -\pi \lt t \lt \frac{-\pi}{2}. \end{cases}</m> See <xref ref="fig_ch-11-09">Figure</xref>.
        </p>
        <figure xml:id="fig_ch-11-08">
          <image width="73%" source="figs/ch-11/ch-11-fig-08.png"/>
        </figure>
        <figure xml:id="fig_ch-11-09">
          {0.5\linewidth}
          <image width="73%" source="figs/ch-11/ch-11-fig-09.png"/>
        </figure>
        <p>
          \solution{ <m>U(t)=\frac{2}{\pi} \sum\limits_{n=1}^{\infty}\frac{1}{2n-1}\sin[(2n-1)t] - \frac{4}{\pi }\sum\limits_{n=1}^{\infty}\frac{1}{2(2n-1)}\sin[2(2n-1)t]</m>,
          where <m>a_n=0</m> for all <m>n</m>,
          and <m>b_{4n}=0</m> for all <m>n</m>. }
        </p>
      </task>
      <task>
        <p>
          <m>U(t)</m>,
          as defined in <xref ref="fig_ch-11-10">Figure</xref>.
        </p>
      </task>
      <task>
        <p>
          <m>U(t)</m>,
          as defined in <xref ref="fig_ch-11-11">Figure</xref>.
        </p>
        <p>
          \solution{ <m>U(t)=\frac{2}{\pi} \sum\limits_{n=1}^{\infty }\frac{1}{2n-1}\sin[(2n-1)t] + \frac{4}{\pi}\sum\limits_{n=1}^{\infty }\frac{1}{2(2n-1)}\sin[2(2n-1)t]</m>,
          where <m>a_n=0</m> for all <m>n</m>,
          and <m>b_{4n}=0</m> for all <m>n</m>. }
        </p>
      </task>
      <task>
        <p>
          Establish Euler's Formula <xref ref="FourierCoeffB"/> for the coefficients <m>\{b_n\}</m>.
        </p>
        <figure xml:id="fig_ch-11-10">
          <image width="73%" source="figs/ch-11/ch-11-fig-10.png"/>
        </figure>
        <figure xml:id="fig_ch-11-11">
          {0.5\linewidth}
          <image width="73%" source="figs/ch-11/ch-11-fig-11.png"/>
        </figure>
      </task>
      <p>
        \end{exercise}
      </p>
    </exercises>
  </subsection>
</section>