<section xml:id="sec_convolution">
  <title>Convolution</title>
  <p>
    Let <m>F(s)</m> and <m>G(s)</m> denote the transforms of <m>f(t)</m> and <m>g(t)</m>,
    respectively.
    Then the inverse of the product
    <m>F(s)G(s)</m> is given by the function
    <m>h(t) =(f\ast g)(t)</m> and is called the convolution of <m>f(t)</m> and <m>g(t)</m> and can be regarded as a generalized product of <m>f(t)</m> and <m>g(t)</m>.
    Convolutions are helpful in solving integral equations.
  </p>
  <theorem xml:id="thm_convolution">
    <title>Convolution Theorem</title>
    <statement>
      <p>
        Let <m>F(s)</m> and <m>G(s)</m> denote the Laplace transforms of <m>f(t)</m> and <m>g(t)</m>,
        respectively.
        Then the product given by <m>H(s)=F(s)G(s)</m> is the Laplace transformation of the convolution of <m>f</m> and <m>g</m>.
        It is denoted by <m>h(t)=(f\ast g)(t)</m>,
        and has the integral representation
        <md>
          <mrow xml:id="convolution1" number="yes">h(t) \amp = (f\ast g)(t) = \int_0^tf(\tau)g(t-\tau)\,d\tau,  \text{ or }</mrow>
          <mrow xml:id="convolution2" number="yes">h(t) \amp = (g\ast f) (t) =\int_0^tg(\tau)f(t-\tau )\,d\tau</mrow>
        </md>.
      </p>
    </statement>
  </theorem>
  <proof>
    <p>
      The following proof is given for the special case when <m>s</m> is a real number.
      The general case is covered in advanced texts.
      Using the dummy variables <m>\sigma</m> and <m>\tau</m> and the integrals defining the transforms,
      we can express their product as
      <me>
        F(s)G(s) = \left[\int_0^{\infty}f(\sigma) e^{-s\sigma}\,d\sigma\right]\left[\int_0^{\infty}g(\tau)e^{-s\tau}\,d\tau\right]
      </me>.
      The product of integrals in this equation can be written as an iterated integral:
      <me>
        F(s)G(s) = \int_0^{\infty}\left[\int_0^{\infty}f(\sigma)e^{-s(\sigma+\tau)}\,d\sigma\right]g(\tau)\,d\tau
      </me>.
      Hold <m>\tau</m> fixed, and use the change of variables
      <m>t=\sigma +\tau</m> and <m>dt=d\sigma</m>.
      Then the inner integral in the equation can be rewritten to obtain
      <md>
        <mrow>F(s)G(s) \amp = \int_0^{\infty}\left[\int_{\tau }^{\infty}f(t-\tau)e^{-st}\,dt\right]g(\tau)\,d\tau</mrow>
        <mrow>\amp = \int_0^{\infty}\left[\int_{\tau }^{\infty}f(t-\tau)g(\tau)e^{-st}dt\right]d\tau</mrow>
      </md>.
    </p>
    <p>
      The region of integration for this last iterated integral is the wedge-shaped region in the
      <m>(t,\tau)</m> plane shown in <xref ref="fig_ch-11-28">Figure</xref>.
      The order of integration in the integral can be reversed to get:
      <me>
        F(s)G(s) = \int_0^{\infty}\left[\int_0^tf(t-\tau)g(\tau)e^{-st}\,d\tau\right]dt
      </me>.
      This equation can be written as
      <md>
        <mrow>F(s)G(s) \amp = \int_0^{\infty}\left[\int_0^tf(t-\tau)g(\tau)\,d\tau\right]e^{-st}\,dt</mrow>
        <mrow>\amp = \mathcal{L}^{-1}\left(\int_0^tf(t-\tau)g(\tau)\,d\tau\right)</mrow>
      </md>,
      which establishes Equation <xref ref="convolution2"/>.
      Since we can interchange the role of the functions <m>f(t)</m> and <m>g(t)</m>, Equation <xref ref="convolution1"/> follows immediately.
    </p>
  </proof>
  <figure xml:id="fig_ch-11-28">
    <caption>The region of integration in the convolution theorem</caption>
    <image width="73%" source="figs/ch-11/ch-11-fig-28.png"/>
  </figure>
  <p>
    <xref ref="table_convolution-properties">Table</xref>
    summarizes some important convolution properties.
  </p>
  <table xml:id="table_convolution-properties">
    <title>Convolution Properties</title>
    <tabular>
      <row bottom="minor">
        <cell></cell>
        <cell></cell>
      </row>
      <row>
        <cell>Commutativity</cell>
        <cell><m>f\ast g=g\ast f</m></cell>
      </row>
      <row>
        <cell>\hdashline
          Distributivity</cell>
        <cell><m>f\ast (g+h) =f\ast g+f\ast h</m></cell>
      </row>
      <row>
        <cell>\hdashline
          Associativity</cell>
        <cell><m>(f\ast g) \ast h=f\ast (g\ast h)</m></cell>
      </row>
      <row>
        <cell>\hdashline
          Zero</cell>
        <cell><m>f\ast 0=0</m></cell>
      </row>
      <row bottom="minor">
        <cell></cell>
        <cell></cell>
      </row>
    </tabular>
  </table>
  <example>
    <statement>
      <p>
        Show that <m>\mathcal{L}^{-1}\left(\frac{2s}{(s^2+1)^2}\right) = t\sin t</m>.
      </p>
      <p>
        Let <m>F(s) = \frac{1}{s^2+1}</m>,
        <m>G(s) =\frac{2s}{s^2+1}, \, f(t) = \sin t, \, g(t) =2\cos t</m>,
        respectively.
        Applying the convolution theorem we get
        <md>
          <mrow>\mathcal{L}^{-1}\left(\frac{1}{s^2+1}\frac{2s}{s^2+1}\right) \amp = \mathcal{L}^{-1}\big(F(s)G(s)\big)</mrow>
          <mrow>\amp = \int_0^t2\sin(t-\tau) \cos \tau\,d\tau</mrow>
          <mrow>\amp = \int_0^t[2\sin t\cos^2\tau -2\cos t\sin \tau \cos \tau]\,d\tau</mrow>
          <mrow>\amp = \left[\sin t(\tau +\sin \tau \cos \tau ) - \cos t\sin^2\tau\right]\Big|_{\tau =0}^{\tau =t}</mrow>
          <mrow>\amp = t\sin t+\sin^2t\cos t-\cos t\sin^2t</mrow>
          <mrow>\amp = t\sin t</mrow>
        </md>.
      </p>
    </statement>
    <solution>
      <p>
      </p>
    </solution>
  </example>
  <example>
    <statement>
      <p>
        Use the convolution theorem to solve the integral equation
        <me>
          f(t) = 2\cos t-\int_0^t(t-\tau)f(\tau)\,d\tau
        </me>
      </p>
      <p>
        Letting <m>F(s) =\mathcal{L}\big(f(t)\big)</m> and using
        <m>\mathcal{L}(t) = \frac{1}{s^2}</m> in the convolution theorem we obtain
        <me>
          F(s) = \frac{2s}{s^2+1} - \frac{1}{s^2}F(s)
        </me>.
        Solving for <m>F(s)</m> we get
        <me>
          F(s) = \frac{2s^3}{(s^2+1)^2} = \frac{2s}{s^2+1} - \frac{2s}{(s^2+1)^2}
        </me>,
        and the solution is
        <me>
          f(t) = 2\cos t - t\sin t
        </me>
      </p>
    </statement>
    <solution>
      <p>
      </p>
    </solution>
  </example>
  <p>
    Engineers and physicists sometimes consider forces that produce large effects that are applied over a very short time interval.
    The force acting at the time an earthquake starts is an example.
    This leads to the idea of a <em>unit impulse function</em> <m>\delta(t)</m>.
    Consider a small positive constant <m>a</m>.
    The function <m>\delta_a(t)</m> is defined by
    <me>
      \delta_a(t) = \begin{cases}\frac{1}{a} \amp  \text{ for }   0\lt t\lt a,\\ 0 \amp  \text{ otherwise } . \end{cases}
    </me>
  </p>
  <p>
    The unit impulse function is obtained by letting the interval width go to zero,
    <em>i.e.</em>,
    <me>
      \delta(t) = \lim_{a \to 0}\delta_a(t)
    </me>
  </p>
  <p>
    <xref ref="fig_ch-11-29">Figure</xref>
    shows the graph of <m>\delta_a(t)</m> for <m>a=10, \, 40</m>,
    and <m>100</m>.
    Although <m>\delta(t)</m> is called the
    <em>Dirac delta function</em>,
    it is not an ordinary function.
    To be precise it is a distribution,
    and the theory of distributions permits manipulations of
    <m>\delta(t)</m> as though it were a function.
    For our work, we will treat
    <m>\delta(t)</m> as a function and investigate its properties.
  </p>
  <figure xml:id="fig_ch-11-29">
    <caption>Graphs of <m>y=\delta_a(t)</m> for <m>a=10</m>, <m>40</m>, and <m>100</m></caption>
    <image width="73%" source="figs/ch-11/ch-11-fig-29.png"/>
  </figure>
  <example>
    <statement>
      <p>
        Show that <m>\mathcal{L}\big(\delta(t)\big) = 1</m>.
      </p>
      <p>
        By definition, the Laplace transform of <m>\delta_a(t)</m> is
        <me>
          \mathcal{L}\big(\delta_a(t)\big) = \int_0^{\infty}\delta_a(t)e^{-st}\,dt = \int_0^{a}\frac{1}{a}e^{-st}\,dt = \frac{1-e^{-sa}}{sa}
        </me>.
      </p>
      <p>
        Letting <m>a \to 0</m> in equation,
        and using L'H&#xf4;pital's rule, we obtain
        <me>
          \mathcal{L}\big(\delta(t)\big) = \lim_{a \to 0}\mathcal{L}\big(\delta_a(t)\big) = \lim\limits_{a \to 0}\frac{1-e^{-sa}}{sa}=\lim\limits_{a \to 0}\frac{0+se^{-sa}}{s} = 1
        </me>.
      </p>
    </statement>
    <solution>
      <p>
      </p>
    </solution>
  </example>
  <p>
    We now turn our attention to the unit impulse function.
    First, consider the function <m>f_a(t)</m> obtained by integrating <m>\delta_a(t)</m>:
    <me>
      f_a(t) = \int_0^t\delta_a(\tau )\,d\tau = \begin{cases}0 \amp  \text{ for }   t \lt  0,\\ \frac{t}{a} \amp  \text{ for }   0 \le t \le a,\\ 1 \amp  \text{ for }   a \lt  t. \end{cases}
    </me>
  </p>
  <p>
    Then it is easy to see that <m>U_0(t) =\lim\limits_{a \to 0}f_a(t)</m>
    (see <xref ref="fig_ch-11-30">Figure</xref>).
  </p>
  <figure xml:id="fig_ch-11-30">
    <caption>The integral of <m>\delta_a(t)</m> is <m>f_a(t)</m>, which becomes <m>U_0(T)</m>, which becomes <m>U_0(t)</m> when <m>a \to 0</m></caption>
    <image width="73%" source="figs/ch-11/ch-11-fig-30.png"/>
  </figure>
  <p>
    The response of a system to the unit impulse function is illustrated in the next example.
  </p>
  <example xml:id="ex_10_32">
    <statement>
      <p>
        Solve the initial value problem
        <me>
          y\,''(t)+4y\,'(t)+13y(t)=3\delta(t) \text{ with }   y(0) =0  \text{ and } y\,'(0^-)=0
        </me>.
      </p>
      <p>
        Taking transforms results in <m>(s^2+4s+13)Y(s) = 3\mathcal{L}(\delta (t)) = 3</m>, so that
        <me>
          Y(s) = \frac{3}{s^2+4s+13}=\frac{3}{(s+2)^2+3^2}
        </me>,
        so the solution is
        <me>
          y(t)=e^{-2t}\sin 3t
        </me>
      </p>
    </statement>
    <solution>
      <p>
      </p>
    </solution>
  </example>
  <p>
    Note: The condition <m>y\,'(0^-) =0</m> is not satisfied by the
    <q>solution</q>
    <m>y(t)</m>.
    Recall that all solutions using the Laplace transform are to be considered zero for values of <m>t\lt 0</m>.
    Hence the graph of <m>y(t)</m> is given in <xref ref="fig_ch-11-31">Figure</xref>.
    We see that <m>y,'(t)</m> has a jump discontinuity of magnitude <m>+3</m> at the origin.
    This happens because either <m>y(t)</m> or <m>y\,'(t)</m> must have a jump discontinuity at the origin whenever the Dirac delta function occurs as part of the input or driving function.
  </p>
  <figure xml:id="fig_ch-11-31">
    <caption>The solution <m>y=y(t)</m> to <xref ref="ex_10_32">Example</xref></caption>
    <image width="73%" source="figs/ch-11/ch-11-fig-31.png"/>
  </figure>
  <p>
    We now illustrate how the convolution method can be used to solve initial value problems.
  </p>
  <example xml:id="thm_convolution-method">
    <title>IVP Convolution Method</title>
    <statement>
      <p>
        Show initial value problem
        <me>
          ay\,''(t) + by\,'(t) + cy(t) = g(t),  \text{ with } y(0) = y_0  \text{ and }   y\,'(0) = y_1
        </me>
        has the unique solution
        <me>
          y(t) = u(t) + (h\ast g)(t)
        </me>,
        where <m>u(t)</m> is the solution to the homogeneous equation
        <me>
          au\,''(t) + bu\,'(t) + cu(t) = 0,  \text{ with } u(0) = y_0  \text{ and }   u'(0) = y_1
        </me>,
        and <m>h(t)</m> is the function whose Laplace transform given by <m>H(s) = \frac{1}{as^2+bs+c}</m>.
      </p>
      <p>
        The particular solution is found by solving the equation
        <me>
          av\,''(t) + bv\,'(t) + cv(t) = g(t),  \text{ with }   v(0) = 0  \text{ and }   v\,'(0) = 0
        </me>.
      </p>
      <p>
        Taking the Laplace transform of both sides of this equation produces
        <me>
          as^2V(s) + bsV(s) + cV(s) = G(s)
        </me>.
        Solving for <m>V(s)</m> in the latter equation yields <m>V(s)=\frac{1}{as^2+bs+c}G(s)</m>.
        If we set <m>H(s) =\frac{1}{as^2+bs+c}</m>,
        then <m>V(s) =H(s)G(s)</m>,
        and the particular solution is given by the convolution
        <me>
          v(t) = (h\ast g)(t)
        </me>.
        The general solution is <m>y(t) = u(t) + v(t) = u(t) + (h\ast g)(t)</m>.
        To verify that the initial conditions are met we compute
        <md>
          <mrow>y(0) \amp = u(0) + v(0) = y_0 + i0 = y_0,  \text{ and }</mrow>
          <mrow>y\,'(0) \amp = u\,'(0) +v\,'(0) = y_1 + 0 = y_1</mrow>
        </md>.
      </p>
    </statement>
    <solution>
      <p>
      </p>
    </solution>
  </example>
  <example>
    <statement>
      <p>
        Use the convolution method to solve the IVP
        <me>
          y\,''(t) + y(t) = \tan t,  \text{ with }   y(0) = 1  \text{ and }   y\,'(0) = 2
        </me>.
      </p>
      <p>
        First solve <m>u''(t) + u(t) = 0</m> with
        <m>u(0) = 1</m> and <m>u'(0) = 2</m>.
        Taking the Laplace transform yields <m>s^2U(s) - s- 2 + U(s) = 0</m>.
        Solving for <m>U(s)</m> gives <m>U(s) = \frac{s+2}{s^2+1}</m>,
        and it follows that
        <me>
          u(t) = \cos t + 2\sin t
        </me>.
        Second, observe that <m>H(s) = \frac{1}{s^2+1}</m> and <m>h(t) = \sin t</m>, so that
        <md>
          <mrow>v(t) \amp = (h\ast g) (t) = \int_0^t\sin(t-s) \tan(s)\,ds</mrow>
          <mrow>\amp = \left.\left[\cos (t) \ln \frac{\cos s}{1+\sin s}-\sin (t-s)\right]\right|_{s=0}^{s=t}</mrow>
          <mrow>\amp = \cos (t) \ln \frac{\cos t}{1+\sin t}+\sin (t)</mrow>
        </md>.
      </p>
      <p>
        Therefore, the solution is
        <me>
          y(t) = u(t) + v(t) = \cos t + 3\sin t + \cos(t) \ln \frac{\cos t}{1+\sin t}
        </me>
      </p>
    </statement>
    <solution>
      <p>
      </p>
    </solution>
  </example>
  <exercises xml:id="exercises_convolution">
    <title>Exercises</title>
    <exercise>
      <introduction>
        <p>
          Find the indicated convolution for each of the following:
        </p>
      </introduction>
      <task>
        <statement>
          <p>
            <m>t\ast t</m>.
          </p>
        </statement>
        <solution>
          <p>
            <m>f(t)=t, \, g(t)=t</m>,
            and <m>(f \ast g)(t) = \int_0^tf(\tau)g(t-\tau)\,d\tau = \int_0^t\tau(t-\tau)\,d\tau = \frac{t^3}{6}</m>.
          </p>
        </solution>
      </task>
      <task>
        <p>
          <m>t\ast \sin t</m>.
        </p>
      </task>
      <task>
        <statement>
          <p>
            <m>e^t\ast e^{2t}</m>.
          </p>
        </statement>
        <solution>
          <p>
            <m>f(t)=e^t, \, g(t)=e^{2t}</m>,
            and <m>(g \ast f)(t) = \int_0^te^{2\tau }e^{t-\tau}\,d\tau = -e^t+e^{2t}</m>.
          </p>
        </solution>
      </task>
      <task>
        <p>
          <m>\sin t\ast \sin 2t</m>.
        </p>
      </task>
    </exercise>
    <exercise>
      <introduction>
        <p>
          Use convolution to find <m>\mathcal{L}^{-1}\big(F(s)\big)</m> for each of the following:
        </p>
      </introduction>
      <task>
        <statement>
          <p>
            <m>F(s) =\frac{2}{(s-1)(s-2)}</m>.
          </p>
        </statement>
        <solution>
          <p>
            <m>f(t)=\mathcal{L}^{-1}\Big(\frac{2}{(s-1)(s-2)}\Big)=-2e^t+2e^{2t}</m>.
          </p>
        </solution>
      </task>
      <task>
        <p>
          <m>F(s) = \frac{6}{s^3}</m>.
        </p>
      </task>
      <task>
        <statement>
          <p>
            <m>F(s) = \frac{1}{s(s^2+1)}</m>.
          </p>
        </statement>
        <solution>
          <p>
            <m>f(t)=\mathcal{L}^{-1}\Big(\frac{1}{s(s^2+1)}\Big) = 1 - \cos t</m>.
          </p>
        </solution>
      </task>
      <task>
        <p>
          <m>F(s) = \frac{s}{(s^2+1)(s^2+4)}</m>.
        </p>
      </task>
    </exercise>
    <exercise>
      <statement>
        <p>
          Prove the distributive law for convolution:
          <m>f\ast (g+h) = f\ast g+f\ast g</m>.
        </p>
      </statement>
      <solution>
        <p>
          Proof: <m>f \ast(g+h) = \int_0^tf(\tau)(g+h)(t-\tau)\,d\tau = \int_0^tf(\tau)g(t-\tau)\,d\tau + \int_{0}^tf(\tau)h(t-\tau )d\tau = f\ast g+f\ast g</m>.
        </p>
      </solution>
    </exercise>
    <exercise>
      <statement>
        <p>
          Use the convolution theorem and mathematical induction to show that
          <me>
            \mathcal{L}^{-1}\left(\frac{1}{(s-a)^n}\right) = \frac{1}{(n-1)!}t^{n-1}e^{at}
          </me>
        </p>
      </statement>
    </exercise>
    <exercise>
      <statement>
        <p>
          Find <m>\mathcal{L}^{-1}(\frac{s}{s-1})</m>.
        </p>
      </statement>
      <solution>
        <p>
          <m>f(t) = \mathcal{L}^{-1}\big(\frac{s}{s-1}) = e^t+\delta (t)</m>.
        </p>
      </solution>
    </exercise>
    <exercise>
      <statement>
        <p>
          Find <m>\mathcal{L}^{-1}(\frac{s^2}{s^2+1})</m>.
        </p>
      </statement>
    </exercise>
    <exercise>
      <statement>
        <p>
          Use the convolution theorem to solve the initial value problem
          <me>
            y\,''(t) +y(t) = 2\sin t,  \text{ with }   y(0) = 0  \text{ and }   y\,'(0) = 0
          </me>.
        </p>
      </statement>
      <solution>
        <p>
          <m>y(t) = -t\cos t+\sin t</m>.
        </p>
      </solution>
    </exercise>
    <exercise>
      <statement>
        <p>
          Use the convolution theorem to show that the solution to the initial value problem
        </p>
        <p>
          <m>y\,''(t) + \omega^2y(t) = f(t)</m>,
          with <m>y(0) = 0</m> and <m>y\,'(0) = 0</m> is
          <me>
            y(t) = \frac{1}{\omega}\int_0^tf(\tau)\sin[\omega(t-\tau )]\,d\tau
          </me>
        </p>
      </statement>
    </exercise>
    <exercise>
      <statement>
        <p>
          Find <m>\mathcal{L}\left(\int_0^te^{-\tau }\cos (t-\tau)\,d\tau\right)</m>.
        </p>
      </statement>
      <solution>
        <p>
          <m>\mathcal{L}\left(\int_{0}^te^{-\tau}\cos(t-\tau)\,d\tau \right) = \mathcal{L}(e^t) \mathcal{L}\big(\cos(t)\big) = \frac{s}{(s+1)(s^2+1)}</m>.
        </p>
      </solution>
    </exercise>
    <exercise>
      <statement>
        <p>
          Find <m>\mathcal{L}\left(\int_0^t(t-\tau )^2e^{\tau}\,d\tau\right)</m>.
        </p>
      </statement>
    </exercise>
    <exercise>
      <statement>
        <p>
          Let <m>F(s) =\mathcal{L}\big(f(t)\big)</m>.
          Use convolution to show that
          <me>
            \mathcal{L}^{-1}\left(\frac{F(s)}{s}\right) = \int_0^tf(\tau)\,d\tau
          </me>
        </p>
      </statement>
      <solution>
        <p>
          Given <m>F(s) = \mathcal{L}\big(f(t)\big)</m> and <m>G(s)=\mathcal{L}(1) = \frac{1}{s}</m> and <m>g(t)=1</m>,
          we have <m>\mathcal{L}^{-1}\left(\frac{F(s)}{s}\right) = F(s)G(s) = (f \ast g)(t) = \int_0^tf(\tau)g(t-\tau)\,d\tau = \int_{0}^tf(\tau)\,d\tau</m>.
        </p>
      </solution>
    </exercise>
    <exercise>
      <introduction>
        <p>
          Use the convolution theorem to solve the following integral equations.
        </p>
      </introduction>
      <task>
        <statement>
          <p>
            <m>f(t) = e^t + \int_0^te^{t-\tau}f(\tau)\,d\tau</m>.
          </p>
        </statement>
        <solution>
          <p>
            <m>F(s) = \frac{1}{s-2}</m>, and <m>f(t)=e^{2t}</m>.
          </p>
        </solution>
      </task>
      <task>
        <p>
          <m>f(t) + 4\int_0^t(t-\tau)f(\tau)\,d\tau = 2</m>.
        </p>
      </task>
      <task>
        <statement>
          <p>
            <m>6f(t) = 2t^3 + \int_0^t(t-\tau)^3f(\tau)\,d\tau</m>.
          </p>
        </statement>
        <solution>
          <p>
            <m>F(s) = \frac{2}{s^{4}-1}</m>,
            and <m>f(t)=\sinh t-\sin t</m>.
          </p>
        </solution>
      </task>
      <task>
        <p>
          <m>f(t) = 2t + \int_0^t\sin(t-\tau)f(\tau)\,d\tau</m>.
        </p>
      </task>
    </exercise>
    <exercise>
      <introduction>
        <p>
          Solve the initial value problem for each of the following:
        </p>
      </introduction>
      <task>
        <statement>
          <p>
            <m>y\,''(t) + 2y\,'(t) + y(t) = \delta(t)</m>,
            with <m>y(0) = 0</m> and <m>y\,'(0) = 0</m>.
          </p>
        </statement>
        <solution>
          <p>
            <m>y(t) = te^{-t}</m>.
          </p>
        </solution>
      </task>
      <task>
        <p>
          <m>y\,''(t) - 2y\,'(t) + 5y(t) = 2\delta(t)</m>,
          with <m>y(0) = 0</m> and <m>y\,'(0) = 0</m>.
        </p>
      </task>
      <task>
        <statement>
          <p>
            <m>y\,''(t) + 4y\,'(t) + 3y(t) = 2\delta(t-1)</m>,
            with <m>y(0) = 0</m> and <m>y\,'(0) = 0</m>.
          </p>
        </statement>
        <solution>
          <p>
            <m>y(t) = (-e^{3-3t} + e^{1-t})U_1(t)</m>.
          </p>
        </solution>
      </task>
      <task>
        <p>
          <m>y\,''(t) + 4y\,'(t) + 3y(t) = 2\delta(t)</m>,
          with <m>y(0) = 0</m> and <m>y\,'(0) = 0</m>.
        </p>
      </task>
    </exercise>
    <exercise>
      <introduction>
        <p>
          Use the IVP convolution method to solve the following initial value problems.
        </p>
      </introduction>
      <task>
        <statement>
          <p>
            <m>y\,''(t) + 2y\,'(t) +y(t) = t^4</m>,
            with <m>y(0) = 1</m> and <m>y\,'(0) = 2</m>.
          </p>
        </statement>
        <solution>
          <p>
            <m>y(t) = -21te^{-t} - 119e^{-t} + 120 - 96t + 36t^2 - 8t^3 + t^4</m>.
          </p>
        </solution>
      </task>
      <task>
        <p>
          <m>y\,''(t) - 2y\,'(t) + 5y(t) = 8\exp(-t)</m>,
          with <m>y(0) = 1</m> and <m>y\,'(0) = 2</m>.
        </p>
      </task>
      <task>
        <p>
          <m>y\,''(t) + 4y\,'(t) + 3y(t) = 24t^2e^{-t}</m>,
          with <m>y(0) = 1</m> and <m>y\,'(0) = 2</m>.
        </p>
      </task>
      <task>
        <p>
          <m>y\,''(t) + 4y\,'(t) + 3y(t) = 2te^{-t}</m>,
          with <m>y(0) = 1</m> and <m>y\,'(0) = 2</m>.
        </p>
      </task>
    </exercise>
  </exercises>
</section>