<section xml:id="sec_mult-and-division-by-t">
  <title>Multiplication and Division by <m>t</m></title>
  <p>
    Sometimes the solutions to nonhomogeneous linear differential equations with constant coefficients involve the functions <m>t\cos bt</m>,
    <m>t\sin bt</m>, or <m>t^ne^{at}</m> as part of the solution.
    We now show how the Laplace transforms of <m>tf(t)</m> and
    <m>\frac{f(t)}{t}</m> are related to the Laplace transform of <m>f(t)</m>.
    The transform of <m>tf(t)</m> will be obtained via differentiation and the transform of
    <m>\frac{f(t)}{t}</m> will be obtained via integration.
    To be precise, we state the following theorems.
  </p>
  <theorem>
    <title>Multiplication by
    <q>$t$</q>
    </title>
    <statement>
      <p>
        If <m>F(s)</m> is the Laplace transform of <m>f(t)</m>, then
        <me>
          \mathcal{L}\big(tf(t)\big) = -F\,'(s)
        </me>
      </p>
    </statement>
  </theorem>
  <proof>
    <p>
      By definition we have <m>F(s) = \int_0^{\infty}f(t)e^{-st}\,dt</m>.
      Leibniz's rule for partial differentiation under the integral sign permits us to write
      <md>
        <mrow>F\,'(s) \amp = \frac{\partial }{\partial s}\int_0^{\infty}f(t)e^{-st}\,dt</mrow>
        <mrow>\amp = \int_0^{\infty}\frac{\partial }{\partial s}[f(t)e^{-st}]\,dt</mrow>
        <mrow>\amp = \int_0^{\infty}[-tf(t) e^{-st}]\,dt</mrow>
        <mrow>\amp = -\int_0^{\infty}tf(t) e^{-st}dt</mrow>
        <mrow>\amp = -\mathcal{L}\big(tf(t)\big) </mrow>
      </md>.
    </p>
  </proof>
  <theorem xml:id="thm_div-by-t">
    <title>Division by $t$</title>
    <statement>
      <p>
        Let both <m>f(t)</m> and <m>\frac{f(t)}{t}</m> have Laplace transforms and let <m>F(s)</m> denote the transform of <m>f(t)</m>.
        If <m>\lim\limits_{t \to 0^+}\frac{f(t)}{t}</m> exists,
        <me>
          \mathcal{L}\left(\frac{f(t)}{t}\right) = \int_s^{\infty}F(\sigma)\,d\sigma
        </me>
      </p>
    </statement>
  </theorem>
  <proof>
    <p>
      Since <m>F(\sigma) = \int_0^{\infty}f(t) e^{-\sigma t}\,dt</m>,
      we integrate <m>F(\sigma)</m> from <m>s</m> to <m>\infty</m>:
      <me>
        \int_s^{\infty}F(\sigma ) d\sigma =\int_0^{\infty}\left[\int_0^{\infty}f(t) e^{-\sigma t}\,dt\right]d\sigma
      </me>.
      The order of integration in equation in the double integral is reversed:
      <md>
        <mrow>\int_s^{\infty}F(\sigma )\,d\sigma \amp = \int_0^{\infty}\left[\int_s^{\infty}f(t) e^{-\sigma t}d\sigma\right]dt</mrow>
        <mrow>\amp = \int_0^{\infty}\left[\frac{-f(t)}{t}e^{-\sigma t}\Big|_{\sigma =s}^{\sigma =\infty}\right]dt</mrow>
        <mrow>\amp = \int_0^{\infty}\frac{f(t)}{t}e^{-st}\,dt</mrow>
        <mrow>\amp = \mathcal{L}\left(\frac{f(t)}{t}\right)</mrow>
      </md>.
    </p>
  </proof>
  <example>
    <statement>
      <p>
        Show that <m>\mathcal{L}(t\cos bt) =\frac{s^2-b^2}{(s^2+b^2)^2}</m>.
      </p>
      <p>
        Let <m>f(t) =\cos bt</m>,
        then <m>F(s) =\mathcal{L}(\cos bt) = \frac{s}{s^2+b^2}</m>.
        Hence, we can differentiate <m>F(s)</m> to obtain the desired result:
        <me>
          \mathcal{L}(t\cos bt) =-F\,'(s) =-\frac{s^2+b^2-2s^2}{(s^2+b^2)^2}=\frac{s^2-b^2}{(s^2+b^2)}
        </me>
      </p>
    </statement>
    <solution>
      <p>
      </p>
    </solution>
  </example>
  <example>
    <statement>
      <p>
        Show that <m>\mathcal{L}(\frac{\sin t}{t}) =\arctan \frac{1}{s}</m>.
      </p>
      <p>
        Let <m>f(t) = \sin t</m> and <m>F(s) =\frac{1}{s^2+1}</m>.
        Since <m>\lim\limits_{t \to 0^+}\frac{\sin t}{t}=1</m>,
        we can integrate <m>F(s)</m> to obtain the desired result:
        <me>
          \mathcal{L}\left(\frac{\sin t}{t}\right) = \int_s^{\infty}\frac{d\sigma}{\sigma^2+1} = \left.-\arctan \frac{1}{\sigma }\right|_{\sigma =s}^{\sigma =\infty} = \arctan \frac{1}{s}
        </me>.
      </p>
    </statement>
    <solution>
      <p>
      </p>
    </solution>
  </example>
  <p>
    Some types of differential equations involve the terms <m>ty\,'(t)</m> or <m>ty\,''(t)</m>.
    Laplace transforms can be used to find the solution if we use the additional substitutions
    <md>
      <mrow xml:id="Laplacety1" number="yes">\mathcal{L}\big(ty\,'(t)\big) \amp = -sY\,'(s) - Y(s),  \text{ and }</mrow>
      <mrow xml:id="Laplacety2" number="yes">\mathcal{L}\big(ty\,''(t)\big) \amp = -s^2Y\,'(s) - 2sY(s) + y(0)</mrow>
    </md>.
  </p>
  <example>
    <statement>
      <p>
        Use Laplace transforms to solve the initial value problem
        <me>
          ty\,''(t) - ty\,'(t) - y(t) = 0  \text{ with }   y(0) =0
        </me>.
      </p>
      <p>
        Let <m>Y(s)</m> denote the Laplace transform of <m>y(t)</m>,
        then using the <xref ref="Laplacety1">substitutions</xref>
        and <xref ref="Laplacety2"></xref> results in
        <men xml:id="LaplaceTransDE">
          -s^2Y\,'(s) -2sY(s) +0+sY\,'(s) + Y(s) - Y(s) = 0
        </men>.
      </p>
      <p>
        This equation involves <m>Y\,'(s)</m> and can be written as a first-order linear differential equation:
        <men xml:id="TransDE">
          Y\,'(s) + \left(\frac{2}{s-1}\right)Y(s) = 0
        </men>.
      </p>
      <p>
        The integrating factor <m>\rho</m> for the differential equation is
        <me>
          \rho = \exp\left(\int \frac{2}{s-1}\,ds\right) = e^{2\ln (s-1)}=(s-1)^2
        </me>.
      </p>
      <p>
        Multiplying Equation <xref ref="TransDE"/> by <m>\rho</m> produces
        <me>
          (s-1)^2Y\,'(s) +2(s-1) Y(s) = \frac{d}{ds}\big[(s-1)^2Y(s)\big] = 0
        </me>.
      </p>
      <p>
        Now we integrate the equation
        <m>\frac{d}{ds}\big[(s-1)^2Y(s)\big] = 0</m> with respect to <m>s</m> and the results is <m>(s-1)^2Y(s) =C</m>,
        where <m>C</m> is the constant of integration.
        Hence the solution to Equation <xref ref="LaplaceTransDE"/> is
        <me>
          Y(s) = \frac{C}{(s-1)^2}
        </me>.
        The inverse of the transform <m>Y(s)</m> in equation is the desired solution
        <me>
          y(t) = Cte^t
        </me>
      </p>
    </statement>
    <solution>
      <p>
      </p>
    </solution>
  </example>
  <exercises xml:id="exercises_mult-and-division-by-t">
    <title>Exercises</title>
    <exercise>
      <introduction>
        <p>
          Find the Laplace transform for each of the following:
        </p>
      </introduction>
      <task>
        <statement>
          <p>
            <m>\mathcal{L}(te^{-2t})</m>.
          </p>
        </statement>
        <solution>
          <p>
            <m>\mathcal{L}(te^{-2t}) = \frac{1}{(s+2)^2}</m>.
          </p>
        </solution>
      </task>
      <task>
        <p>
          <m>\mathcal{L}(t^2e^{4t})</m>.
        </p>
      </task>
      <task>
        <statement>
          <p>
            <m>\mathcal{L}(t\sin 3t)</m>.
          </p>
        </statement>
        <solution>
          <p>
            <m>\mathcal{L}(t\sin 3t) = \frac{6s}{(s^2+9)^2}</m>.
          </p>
        </solution>
      </task>
      <task>
        <p>
          <m>\mathcal{L}(t^2\cos 2t)</m>.
        </p>
      </task>
      <task>
        <statement>
          <p>
            <m>\mathcal{L}(t\sinh t)</m>.
          </p>
        </statement>
        <solution>
          <p>
            <m>\mathcal{L}(t\sinh t) = \frac{2s}{(s^2-1)^2}</m>.
          </p>
        </solution>
      </task>
      <task>
        <p>
          <m>\mathcal{L}(t^2\cosh t)</m>.
        </p>
      </task>
    </exercise>
    <exercise>
      <statement>
        <p>
          Show that <m>\mathcal{L}(\frac{1-\cos t}{t}) = \ln \frac{s^2}{s^2+1}</m>.
        </p>
      </statement>
    </exercise>
    <exercise>
      <statement>
        <p>
          Show that <m>\mathcal{L}(\frac{e^t-1}{t}) = \ln \frac{s}{s-1}</m>.
        </p>
      </statement>
    </exercise>
    <exercise>
      <statement>
        <p>
          Find <m>\mathcal{L}(te^{at}\cos bt)</m>.
        </p>
      </statement>
    </exercise>
    <exercise>
      <statement>
        <p>
          Find <m>\mathcal{L}(t\sin bt)</m>.
        </p>
      </statement>
      <solution>
        <p>
          <m>\mathcal{L}(t\sin bt) = \frac{2bs}{(s^2+b^2)^2}</m>.
        </p>
      </solution>
    </exercise>
    <exercise>
      <statement>
        <p>
          Find <m>\mathcal{L}^{-1}(\ln \frac{s}{s+1})</m>.
        </p>
      </statement>
    </exercise>
    <exercise>
      <statement>
        <p>
          Find <m>\mathcal{L}^{-1}\big(\ln \frac{s^2+1}{(s-1)^2}\big)</m>.
        </p>
      </statement>
      <solution>
        <p>
          <m>\mathcal{L}^{-1}\Big(\ln \frac{s^2+1}{(s-1)^2}\Big) = \frac{2(e^t-\cos t)}{t}</m>.
        </p>
      </solution>
    </exercise>
    <exercise>
      <introduction>
        <p>
          Solve the initial value problem for each of the following:
        </p>
      </introduction>
      <task>
        <statement>
          <p>
            <m>y\,''(t) +2y\,'(t) + y(t) = 2e^{-t}</m>,
            with <m>y(0) = 0</m> and <m>y\,'(0) = 1</m>.
          </p>
        </statement>
        <solution>
          <p>
            <m>y(t) = te^{-t}+t^2e^{-t}</m>.
          </p>
        </solution>
      </task>
      <task>
        <p>
          <m>y\,''(t) + y(t) = 2\sin t</m>,
          with <m>y(0) = 0</m> and <m>y\,'(0) = -1</m>.
        </p>
      </task>
      <task>
        <statement>
          <p>
            <m>ty\,''(t) - ty\,'(t) - y(t) = 0</m>, with <m>y(0) = 0</m>.
          </p>
        </statement>
        <solution>
          <p>
            <m>y(t) = Cte^t</m>.
          </p>
        </solution>
      </task>
      <task>
        <p>
          <m>ty\,''(t) + (t-1)y\,'(t) - 2y(t) = 0</m>, with <m>y(0) = 0</m>.
        </p>
      </task>
      <task>
        <statement>
          <p>
            <m>ty\,''(t) + ty\,'(t) - y(t) = 0</m>, with <m>y(0) = 0</m>.
          </p>
        </statement>
        <solution>
          <p>
            <m>y(t) = Ct</m>.
          </p>
        </solution>
      </task>
      <task>
        <p>
          <m>ty\,''(t) + (t-1)y\,'(t) + y(t) = 0</m>, with <m>y(0) = 0</m>.
        </p>
      </task>
    </exercise>
    <exercise>
      <statement>
        <p>
          Solve the Laguerre equation
          <m>ty\,''(t) + (1-t)y\,'(t) + y(t) = 0</m>, with <m>y(0) = 1</m>.
        </p>
      </statement>
      <solution>
        <p>
          <m>y(t) = 1-t</m>.
        </p>
      </solution>
    </exercise>
    <exercise>
      <statement>
        <p>
          Solve the Laguerre equation
          <m>ty\,''(t) + (1-t)y\,'(t) + 2y(t) = 0</m>, with <m>y(0) = 1</m>.
        </p>
      </statement>
    </exercise>
  </exercises>
</section>