<section xml:id="sec_power-series">
  <title>Power Series Functions</title>
  <p>
    Suppose that we have a series <m>\sum\limits_{n=0}^{\infty}\zeta_n</m>,
    where <m>\zeta_n=c_n(z-\alpha )^n</m>.
    If <m>\alpha</m> and the collection of <m>c_n</m> are fixed complex numbers,
    we get different series by selecting different values for <m>z</m>.
    For example,
    if <m>\alpha =2</m> and <m>c_n=\frac{1}{n!}</m> for all <m>n</m>,
    we get the series <m>\sum\limits_{n=0}^{ \infty}\frac{1}{n!}(\frac{i}{2}-2)^n</m> if
    <m>z=\frac{i}{2}</m> and <m>\sum\limits_{n=0}^{\infty}\frac{1}{n!}(2+i)^n</m> if <m>z=4+i</m>.
    Note that, when <m>\alpha =0</m> and <m>c_n=1</m> for all <m>n</m>,
    we get the geometric series.
    The collection of points for which the series
    <m>\sum\limits_{n=0}^{ \infty}c_n(z-\alpha )^n</m> converges is the domain of a function <m>f(z) =\sum\limits_{n=0}^{\infty}c_n(z-\alpha)^n</m>,
    which we call a <term>power series function</term>.
    Technically, this series is undefined if
    <m>z=\alpha</m> and <m>n=0</m> because <m>0^{0}</m> is undefined.
    We get around this difficulty by stipulating that the series
    <m>\sum\limits_{n=0}^{\infty}c_n(z-\alpha )^n</m> is really compact notation for <m>c_0+\sum\limits_{n=1}^{\infty}c_n( z-\alpha)^n</m>.
    In this section we present some results that are useful in helping establish properties of functions defined by power series.
  </p>
  <theorem xml:id="Regions_of_Convergence">
    <statement>
      <p>
        Suppose that <m>f(z)=\sum\limits_{n=0}^{\infty}c_n(z-\alpha )^n</m>.
        Then the set of points <m>z</m> for which the series converges is one of the following:
        <ol>
          <li>
            <title>i</title>
            <p>
              the single point <m>z=\alpha</m>;
            </p>
          </li>
          <li>
            <title>ii</title>
            <p>
              the disk <m>D_{\rho}(\alpha ) =\{z:|z-\alpha |\lt \rho \}</m>,
              along with part
              (either none, some, or all)
              of the circle <m>C_{\rho}(\alpha ) =\{z:|z-\alpha|=\rho\}</m>;
            </p>
          </li>
          <li>
            <title>iii</title>
            <p>
              the entire complex plane.
            </p>
          </li>
        </ol>
      </p>
    </statement>
  </theorem>
  <proof>
    <p>
      By <xref ref="Root_Test">Theorem</xref>,
      the series converges absolutely at those values of <m>z</m> for which <m>\lim\limits_{n \to \infty}\sup |c_n(z-\alpha )^n|^{\frac{1}{n}}\lt 1</m>.
      This condition is the same as requiring
      <men xml:id="lim_sup_inequality">
        |z-\alpha| \left(\lim_{n \to \infty }\sup |c_n|^{\frac{1}{n}}\right)\lt 1
      </men>.
    </p>
    <p>
      There are three possibilities to consider for the value of <m>\lim\limits_{n \to \infty}\sup |c_n|^{\frac{1}{n}}</m>.
      If the limit supremum equals <m>\infty</m>,
      <xref ref="lim_sup_inequality">Inequality</xref>
      holds iff <m>z=\alpha</m>, which is case
      (<em>i</em>).
      If <m>0\lt \lim\limits_{n \to \infty}\sup |c_n|^{\frac{1}{n}}\lt \infty</m>,
      <xref ref="lim_sup_inequality">Inequality</xref>
      holds iff <m>|z-\alpha |\lt \frac{{1}}{{\lim\limits_{n \to \infty}\sup |c_n|^{\frac{1}{n}}}}</m> (<em>i.e.</em>,
      iff <m>z\in D_{\rho}(\alpha)</m>,
      where <m>\rho =\frac{{1}}{{\lim\limits_{n \to \infty}\sup |c_n|^{\frac{1}{n}}}}</m>) which is case
      (<em>ii</em>).
      Finally, if the limit supremum equals 0, the left side of <xref ref="lim_sup_inequality">Inequality</xref>
      will be 0 for any value of <m>z</m>, which is case
      (<em>iii</em>).
      We are unable to say for sure what happens with respect to convergence on <m>C_{\rho}(\alpha ) =\{z:|z-\alpha|= \rho \}</m>.
      You will see in the exercises that there are various possibilities.
    </p>
  </proof>
  <p>
    Another way to phrase case (<em>ii</em>) of <xref ref="Regions_of_Convergence">Theorem</xref>
    is to say that the power series <m>f(z) =\sum\limits_{n=0}^{\infty}c_n(z-\alpha )^n</m> converges if
    <m>|z-\alpha|\lt \rho</m> and diverges if <m>|z-\alpha|>\rho</m>.
    We call the number <m>\rho</m> the
    <term>radius of convergence</term> of the power series
    (see <xref ref="fig_ch-04-03">Figure</xref>).
    For case (<em>i</em>) of Theorem 4.14,
    we say that the radius of convergence is zero and that the radius of convergence is infinity for case
    (<em>iii</em>).
  </p>
  <figure xml:id="fig_ch-04-03">
    <caption>The radius of convergence of a power series</caption>
    <image width="50%" source="figs/ch-04/ch-04-fig-03.pdf"/>
  </figure>
  <theorem xml:id="th15">
    <statement>
      <p>
        For the power series function
        <m>f(z)=\sum\limits_{n=0}^{\infty}c_n(z-\alpha )^n</m> we can find <m>\rho</m>,
        its radius of convergence, by any of the following methods:
        <ol>
          <li>
            <title>i</title>
            <p>
              Cauchy's root test:
              <m>\rho =\frac{1}{\lim\limits_{n \to \infty}|c_n|^{\frac{1}{n}}}</m>
              (provided the limit exists).
            </p>
          </li>
          <li>
            <title>ii</title>
            <p>
              Cauchy-Hadamard formula:
              <m>\rho =\frac{1}{\lim\limits_{n \to \infty}\sup |c_n|^{\frac{1}{n}}}</m>
              (this limit always exists).
            </p>
          </li>
          <li>
            <title>iii</title>
            <p>
              d'Alembert's ratio test:
              <m>\rho =\frac{1}{\lim\limits_{n\to \infty}|\frac{{c_{n+1}}}{{c_n}}|}</m>
              (provided the limit exists).
            </p>
          </li>
        </ol>
      </p>
      <p>
        We set <m>\rho =\infty</m> if the limit equals 0 and <m>\rho =0</m> if the limit equals <m>\infty</m>.
      </p>
    </statement>
  </theorem>
  <proof>
    <p>
      If you examine carefully the proof of <xref ref="Regions_of_Convergence">Theorem</xref>,
      you will see that we have already proved (<em>i</em>) and
      (<em>ii</em>).
      They follow directly from <xref ref="lim_sup_inequality">Inequality</xref>
      and the fact that the limit supremum equals the limit whenever the limit exists.
      We can show (<em>iii</em>) by using the ratio test.
      We leave the details as an exercise.
    </p>
  </proof>
  <p>
    We now give an example illustrating each of these cases.
  </p>
  <example>
    <statement>
      <p>
        The series <m>\sum\limits_{n=0}^{\infty}(\frac{n+2}{3n+1})^n(z-4)^n</m> has radius of convergence 3 by Cauchy's root test because <m>\lim\limits_{n \to \infty}|c_n|^{\frac{1}{n}}=\lim\limits_{n \to \infty}\frac{n+2}{ 3n+1}=\frac{1}{3}</m>.
      </p>
    </statement>
  </example>
  <example>
    <statement>
      <p>
        The series <m>\sum\limits_{n=1}^{\infty}c_nz^n=4z+5^2z^2+4^{3}z^3+5^{4}z^{4}+4^{5}z^{5}+\cdots</m> has radius of convergence
        <m>\frac{1}{5}</m> by the Cauchy-Hadamard formula because <m>\{|c_n|^{\frac{1}{n}}\} =\{ 4,\,5,\,4,\,5,\ldots \}</m>,
        so <m>\lim\limits_{n \to \infty}\sup |c_n|^{\frac{1}{n}}=5</m>.
      </p>
    </statement>
  </example>
  <example xml:id="e_z_Example">
    <statement>
      <p>
        The series <m>\sum\limits_{n=0}^{\infty}\frac{1}{n!}z^n</m> has radius of convergence <m>\infty</m> by the ratio test because <m>\lim\limits_{n \to \infty}|\frac{n!}{(n+1) !} |=\lim\limits_{n \to \infty}|\frac{1}{n+1}|=0</m>.
      </p>
    </statement>
  </example>
  <p>
    We come now to the main result of this section.
  </p>
  <theorem xml:id="Power_Series_Thm">
    <statement>
      <p>
        <em>Suppose that the function</em><m>f(z)=\sum\limits_{n=0}^{\infty}c_n(z-\alpha )^n</m> has radius of convergence <m>\rho >0</m>.
        Then
        <ol>
          <li>
            <title>i</title>
            <p>
              <m>f</m><nbsp/>is infinitely differentiable for all <m>z\in D_{\rho}(\alpha )</m>.
              In fact
            </p>
          </li>
          <li>
            <title>ii</title>
            <p>
              for all <m>k</m>,
              <m>f^{(k)}(z)=\sum\limits_{n=k}^{\infty}n(n-1) \cdots (n-k+1)c_n(z-\alpha ) ^{n-k}</m>; and
            </p>
          </li>
          <li>
            <title>iii</title>
            <p>
              <m>c_{k}=\frac{f^{(k)}(\alpha )}{k!}</m>,
              where <m>f^{(k)}</m><nbsp/>denotes the <m>k</m>th derivative of <m>f</m>. (When <m>k=0</m>,
              <m>f^{(k)}</m> denotes the function <m>f</m><nbsp/>itself so that
              <m>f^{(0)}(z) =f(z)</m><nbsp/>for all <m>z</m>.)
            </p>
          </li>
        </ol>
      </p>
    </statement>
  </theorem>
  <proof>
    <p>
      Remarkably, the entire proof hinges on verifying (<em>ii</em>) for the simple case when <m>k=1</m>.
      The cases in (<em>ii</em>) for <m>k\ge 2</m> follow by induction.
      For instance,
      we get the case when <m>k=2</m> by applying the result for <m>k=1</m> to the series <m>f\,'(z) =\sum\limits_{n=1}^{\infty}nc_n(z-\alpha ) ^{n-1}</m>.
      Also, ( <em>i</em>) is an automatic consequence of (<em>ii</em>),
      because (<em>ii</em>) gives a formula for computing derivatives of all orders in addition to assuring us of their existence.
      Finally, (<em>iii</em>) follows by setting <m>z=\alpha</m> in (<em>ii</em>),
      as all the terms drop out except when <m>n=k</m>,
      giving us <m>f^{(k)}(\alpha ) =k(k-1) \cdots (k-k+1) c_{k}</m>.
      Solving for <m>c_{k}</m> gives the desired result.
    </p>
    <p>
      Verifying (<em>ii</em>) when <m>k=1</m>,
      however, is no simple task.
      We begin by defining the following functions:
      <md>
        <mrow>g(z) \amp = \sum_{n=1}^{\infty}nc_n(z-\alpha)^{n-1}</mrow>
        <mrow>S_{j}(z) \amp = \sum_{n=0}^{j}c_n(z-\alpha )^n\text{,}</mrow>
        <mrow>R_{j}(z) \amp = \sum_{n=j+1}^{\infty}c_n(z-\alpha)^n</mrow>
      </md>.
    </p>
    <p>
      Here <m>S_{j}(z)</m> is simply the <m>(j+1)</m>st partial sum of the series <m>f(z)</m>,
      and <m>R_{j}(z)</m> is the sum of the remaining terms of that series.
      We leave as an exercise to show that the radius of convergence for <m>g(z)</m> is <m>\rho</m>,
      the same as that of <m>f(z)</m>.
      For a fixed <m>z_0\in D_{\rho}(\alpha)</m>,
      we must prove that <m>f\,'(z_0)=g(z_0)</m>;
      that is, we must prove that <m>\lim_{z \to z_0} \frac{f(z) -f(z_0)}{z-z_0}=g(z_0)</m>.
      We do so by showing that for all
      <m>\varepsilon>0</m> there exists <m>\delta >0</m> such that,
      if <m>z\in D_{\rho}(\alpha )</m> with <m>0\lt | z-z_0|\lt \delta</m>,
      then <m>|\frac{f(z) -f(z_0)}{z-z_0}-g(z_0)| \lt \varepsilon</m>.
    </p>
    <p>
      Let <m>z_0\in D_{\rho}(\alpha )</m> and <m>\varepsilon>0</m> be given.
      Choose <m>r\lt \rho</m> so that <m>z_0\in D_{r}(\alpha)</m>.
      We choose <m>\delta</m> to be small enough so that <m>D_{\delta}(z_0) \subset D_{r}(\alpha) \subset D_{\rho}(\alpha)</m>
      (see <xref ref="fig_ch-04-04">Figure</xref>)
      and also small enough to satisfy an additional restriction,
      which we shall specify in a moment.
    </p>
    <figure xml:id="fig_ch-04-04">
      <caption>Choosing <m>\delta</m> to prove that <m>f\ '(z_0) =g(z_0)</m></caption>
      <image width="73%" source="figs/ch-04/ch-04-fig-04.pdf"/>
    </figure>
    <p>
      Because <m>f(z) =S_{j}(z) +R_{j}(z)</m>,
      simplifying the right side of the following equation reveals that for all <m>j</m>,
      <md>
        <mrow>\left[\frac{f(z) -f(z_0)}{z-z_0}-g(z_0)\right] \amp = \left[\frac{S_{j}(z) -S_{j}(z_0)}{z-z_0}-S_{j}^{\,\prime}(z_0) \right]</mrow>
        <mrow xml:id="x3_parts" number="yes">\amp + \left[ S_{j}^{\,\prime}(z_0) -g(z_0) \right] + \left[ \frac{R_{j}(z) -R_{j}(z_0)}{z-z_0}\right]</mrow>
      </md>,
      where <m>S_{j}^{\,\prime}(z_0)</m> is the derivative of the function <m>S_{j}</m> evaluated at <m>z_0</m>.
      Equation <xref ref="x3_parts"/> has the general form <m>A=B+C+D</m>.
      By the triangle inequality,
      <me>
        |A|=|B+C+D|\le |B|+|C|+|D|
      </me>,
      so our proof will be complete if we can show that for a small enough value of <m>\delta</m>,
      each of the expressions <m>|B|, \, |C|</m>,
      and <m>|D|</m> is less than <m>\frac{\varepsilon}{3}</m>.
    </p>
    <p>
      <em>Calculation for</em><m>|D|</m>
      <md>
        <mrow>\left|\frac{R_{j}(z) -R_{j}(z_0)}{z-z_0}\right| \amp =\left|\frac{1}{z-z_0}\left(\sum\limits_{n=j+1}^{\infty}c_n[(z-\alpha)^n-(z_0-\alpha)^n]\right) \right|</mrow>
        <mrow>\amp \lt  \sum\limits_{n=j+1}^{\infty}|c_n|\left|\frac{(z-\alpha )^n-(z_0-\alpha )^n}{z-z_0}\right|</mrow>
      </md>,
      where the last inequality follows from <xref ref="x4_1_12">Exercise</xref>,
      <xref ref="sec_sequences-series">Section</xref>.
    </p>
    <p>
      As an exercise, we ask you to show that
      <men xml:id="Exercise_Ineq">
        \left|\frac{(z-\alpha )^n-(z_0-\alpha) ^n}{z-z_0}\right| \lt  nr^{n-1}
      </men>.
    </p>
    <p>
      Assuming this to be the case, we get
      <men xml:id="Rj_ineq">
        \left|\frac{R_{j}(z) -R_{j}(z_0)}{z-z_0}\right| \lt  \sum_{n=j+1}^{\infty}|c_n| nr^{n-1}\text{.}
      </men>
    </p>
    <p>
      Since <m>r\lt \rho</m>,
      the series <m>\sum\limits_{n=1}^{\infty}| c_n|nr^{n-1}</m> converges
      (can you explain why?).
      Thus the tail part of the series,
      which is the right side of <xref ref="Rj_ineq">Inequality</xref>,
      can certainly be made less than
      <m>\frac{\varepsilon}{3}</m> if we choose <m>j</m> large enough<mdash/>say,
      <m>j\ge N_1</m>.
    </p>
    <p>
      <em>Calculation for</em> <m>|C|</m>
    </p>
    <p>
      Since <m>S_{j}^{\,\prime}(z_0)=\sum\limits_{n=1}^{j}nc_n(z_0-\alpha ) ^{n-1}</m>,
      it is clear that <m>\lim_{j \to \infty}S_{j}^{\,\prime}(z_0) = g(z_0)</m>.
      Thus there is an integer <m>N_2</m> such that if <m>j \ge N_2</m>,
      then <m>|S_{j}^{\,\prime}(z_0) -g(z_0)|\lt \frac{\varepsilon}{3}</m>.
    </p>
    <p>
      <em>Calculation for</em><m>|B|</m>
    </p>
    <p>
      We define <m>N=\max \{N_1\text{,} N_2\}</m>.
      Because <m>S_{N}(z)</m> is a polynomial,
      <m>S_{N}^{\,\prime}(z_0)</m> exists.
      This means we can find <m>\delta</m> small enough that it complies with the restriction previously placed on it as well as ensuring that
      <me>
        |\frac{S_{N}(z) -S_{N}(z_0)}{z-z_0}-S_{N}^{\,\prime}(z_0)|\lt \frac{\varepsilon}{3}
      </me>
      whenever <m>z\in D_{\rho}(\alpha)</m>,
      with <m>0\lt |z-z_0|\lt \delta</m>.
      Using this value of <m>N</m> for <m>j</m> in Equation <xref ref="x3_parts"/>, together with our chosen <m>\delta</m>,
      yields conclusion (<em>ii</em>) and hence the entire theorem.
    </p>
  </proof>
  <example xml:id="ex_4_24">
    <statement>
      <p>
        Show that <m>\sum\limits_{n=0}^{\infty}(n+1) z^n=\frac{1}{(1-z)^2}</m> for all <m>z\in D_1(0)</m>.
      </p>
    </statement>
    <solution>
      <p>
        We know from <xref ref="Geometric_Series">Theorem</xref>
        that <m>f(z) =\frac{1}{1-z}=\sum\limits_{n=0}^{\infty}z^n</m> for all <m>z\in D_1(0)</m>.
        If we set <m>k=1</m> in Theorem 4.16, part (ii),
        then <m>f\,'(z) = \frac{1}{(1-z)^2} = \sum\limits_{n=1}^{\infty}nz^{n-1} = \sum\limits_{n=0}^{\infty}(n+1)z^n</m>,
        for all <m>z \in D_1(0)</m>.
      </p>
    </solution>
  </example>
  <example xml:id="Bessel_Ex">
    <statement>
      <p>
        The Bessel function of order zero is defined by
        <me>
          J_0(z) =\sum\limits_{n=0}^{\infty}\frac{(-1)^n }{(n!)^2}\left(\frac{z}{2}\right)^{\!2n} = 1-\frac{z^2}{2^2} + \frac{z^4}{2^4 4^4}-\frac{z^6}{2^2 4^2 6^2} + \cdots
        </me>,
        and termwise differentiation shows that its derivative is
        <me>
          J_0^{\,\prime}(z) = \sum_{n=0}^{\infty}\frac{(-1)^{n+1}}{n!(n+1)!}\left(\frac{z}{2}\right)^{\!2n+1} =\frac{-z}{2}+\frac{1}{1!2!}\left(\frac{z}{2}\right)^{\!3}-\frac{1}{2!3!}\left(\frac{z}{2}\right)^{\!5}+\cdots
        </me>.
      </p>
      <p>
        We leave as an exercise to show that the radius of convergence of these series is infinity.
        The Bessel function <m>J_1(z)</m> of order 1 is known to satisfy the differential equation <m>J_1(z) =-J_0^{\,\prime}(z)</m>.
      </p>
    </statement>
  </example>
  <exercises>
    <title>Exercises for <xref ref="sec_power-series">Section</xref></title>
    <exercise xml:id="x4_4_1">
      <p>
        Prove part (<em>iii</em>) of <xref ref="th15">Theorem</xref>.
      </p>
    </exercise>
    <exercise xml:id="x4_4_2">
      <p>
        Consider the series <m>\sum\limits_{n=0}^{\infty}z^n</m>,
        <m>\sum\limits_{n=1}^{\infty}\frac{z^n}{n^2}</m>,
        and <m>\sum\limits_{n=1}^{\infty}\frac{z^n}{n}</m>.
      </p>
      <ol>
        <li>
          <p>
            Show that each series has radius of convergence 1.
          </p>
        </li>
        <li>
          <p>
            Show that the first series converges nowhere on <m>C_1(0) =\{z:|z|=1\}</m>.
          </p>
        </li>
        <li>
          <p>
            Show that the second series converges everywhere on <m>C_1(0)</m>.
          </p>
        </li>
        <li>
          <p>
            It turns out that the third series converges everywhere on <m>C_1(0)</m>,
            except at the point <m>z=1</m>.
            This is not easy to prove.
            Give it a try.
          </p>
        </li>
      </ol>
    </exercise>
    <exercise xml:id="x4_4_3">
      <p>
        Find the radius of convergence of the following.
        <ol>
          <li>
            <p>
              <m>g(z) = \sum\limits_{n=0}^{\infty}(-1)^n \frac{z^n}{(2n)!}</m>.
            </p>
          </li>
          <li>
            <p>
              <m>h(z) = \sum\limits_{n=0}^{\infty}n!z^n</m>.
            </p>
          </li>
          <li>
            <p>
              <m>f(z) = \sum\limits_{n=0}^{\infty}(\frac{4n^2}{2n+1}-\frac{6n^2}{3n+4})^nz^n</m>.
            </p>
          </li>
          <li>
            <p>
              <m>g(z) = \sum\limits_{n=0}^{\infty}\frac{(n!)^2}{(2n)!}z^n</m>.
            </p>
          </li>
          <li>
            <p>
              <m>h(z) = \sum\limits_{n=0}^{\infty}(2-(-1)^n)^nz^n</m>.
            </p>
          </li>
          <li>
            <p>
              <m>f(z) = \sum\limits_{n=0}^{\infty}\frac{n(n-1)z^n}{(3+4i)^n}</m>.
            </p>
          </li>
          <li>
            <p>
              <m>g(z) =\sum\limits_{n=0}^{\infty}(\frac{3n+7}{4n+2}^nz^n</m>.
            </p>
          </li>
          <li>
            <p>
              <m>h(z) = \sum\limits_{n=0}^{\infty}\frac{2^n}{1+3^n}z^n</m>.
            </p>
          </li>
          <li>
            <p>
              <m>g(z) = \sum\limits_{n=0}^{\infty}z^{2n}</m>.
            </p>
          </li>
          <li>
            <p>
              <m>g(z) = \sum\limits_{n=0}^{\infty}\frac{n^n}{n!}z^n</m>.
              <em>Hint</em>:
              <m>\lim\limits_{n \to \infty}(1+\frac{1}{n})^n=e</m>.
            </p>
          </li>
        </ol>
      </p>
    </exercise>
    <exercise xml:id="x4_4_4">
      <p>
        Show that <m>\sum\limits_{n=0}^{\infty}(n+1)^2z^n=\frac{1+z}{(1-z) ^{3}}</m>.
        For what values of <m>z</m> is this valid?
      </p>
    </exercise>
    <exercise xml:id="x4_4_5">
      <p>
        Suppose that <m>\sum\limits_{n=0}^{\infty}c_nz^n</m> has radius of convergence <m>R</m>.
        Show that <m>\sum\limits_{n=0}^{\infty}c_n^2z^n</m> has radius of convergence <m>R^2</m>.
      </p>
    </exercise>
    <exercise xml:id="x4_4_6">
      <p>
        Does there exist a power series
        <m>\sum\limits_{n=0}^{\infty}c_nz^n</m> that converges at <m>z_1=4-i</m> and diverges at <m>z_2=2+3i</m>?
        Why or why not?
      </p>
    </exercise>
    <exercise xml:id="x4_4_7">
      <p>
        Verify part (<em>ii</em>) of <xref ref="Power_Series_Thm">Theorem</xref>
        for all <m>k</m> by using mathematical induction.
      </p>
    </exercise>
    <exercise xml:id="x4_4_8">
      <p>
        This exercise establishes that the radius of convergence for <m>g</m> given in <xref ref="Power_Series_Thm">Theorem</xref> is <m>\rho</m>,
        the same as that of the function <m>f</m>.
        <ol>
          <li>
            <p>
              Explain why the radius of convergence for <m>g</m> is <m>\frac{1}{\lim\limits_{n \to \infty}\sup |nc_n|^{\frac{{1}}{n-1}}}</m>.
            </p>
          </li>
          <li>
            <p>
              Show that <m>\lim\limits_{n \to \infty}\sup | n|^{\frac{{1}}{n-1}}=1</m>.
              <em>Hint</em>: The <m>\lim \sup</m> equals the limit.
              Show that <m>\lim\limits_{n \to \infty}\frac{\log n}{n-1}=0</m>.
            </p>
          </li>
          <li>
            <p>
              Assuming that <m>\lim_{n \to \infty}\sup |c_n|^{\frac{{1}}{n-1}}=\lim_{n \to \infty}\sup|c_n|^{\frac{{1}}{n}}</m>,
              show that the conclusion for this exercise follows.
            </p>
          </li>
          <li>
            <p>
              Verify the truth of the assumption made in part (c).
            </p>
          </li>
        </ol>
      </p>
    </exercise>
    <exercise xml:id="x4_4_9">
      <p>
        Here we establish the validity of <xref ref="Exercise_Ineq">Inequality</xref>
        in the proof of <xref ref="Power_Series_Thm">Theorem</xref>.
        <ol>
          <li xml:id="x4_4_9a">
            <p>
              Show that
              <md>
                <mrow>\left|\frac{s^n-t^n}{s-t}\right| \amp = |s^{n-1}+s^{n-2}t+s^{n-3}t^2+\cdots +st^{n-2}+t^{n-1}|</mrow>
                <mrow>\amp \le |s^{n-1}|+|s^{n-2}t| +|s^{n-3}t^2|+\cdots +|st^{n-2}| +|t^{n-1}|</mrow>
              </md>,
              where <m>s</m> and <m>t</m> are arbitrary complex numbers,
              <m>s \ne t</m>.
            </p>
          </li>
          <li xml:id="x4_4_9b">
            <p>
              Explain why, in <xref ref="Exercise_Ineq">Inequality</xref>,
              <m>|z-\alpha|\lt r</m> and <m>|z_0-\alpha|\lt r</m>.
            </p>
          </li>
          <li xml:id="x4_4_9c">
            <p>
              Let <m>s=z-\alpha</m> and <m>t=z_0-\alpha</m> in part (a) to establish <xref ref="Exercise_Ineq">Inequality</xref>.
            </p>
          </li>
        </ol>
      </p>
    </exercise>
    <exercise xml:id="x4_4_10">
      <p>
        Show that the radius of convergence of the series for <m>J_0(z)</m> and
        <m>J_0^{\,\prime}(z)</m> in <xref ref="Bessel_Ex">Example</xref> is infinity.
      </p>
    </exercise>
    <exercise xml:id="x4_4_11">
      <p>
        Consider the series obtained by substituting for the complex number <m>z</m> the real number <m>x</m> in the Maclaurin series for <m>\sin x</m>.
        Where does this series converge?
      </p>
    </exercise>
    <exercise>
      <p>
        Show that, for <m>|z-i|\lt \sqrt{2}</m>,
        <m>\frac{1}{1-z} =\sum\limits_{n=0}^{\infty}\frac{(z-i)^n}{(1-i) ^{n+1}}</m>.
        <em>Hint</em>:
        <m>\frac{1}{1-z}=\frac{1}{(1-i) -(z-i)}=\frac{1 }{1-i}\Big[\frac{1}{1-\frac{z-i}{1-i}}\Big]</m>.
        Now use <xref ref="Geometric_Series">Theorem</xref>.
      </p>
    </exercise>
  </exercises>
</section>