<section xml:id="sec_laplace-inversion">
  <title>Inverting the Laplace Transform</title>
  <p>
    So far, most of the applications involving the Laplace transform involve a transform
    (or part of a transform)
    that is expressed by
    <men xml:id="quotientPQ">
      Y(s) = \frac{P(s)}{Q(s)}
    </men>.
    where <m>P</m> and <m>Q</m> are polynomials that have no common factors.
    The inverse of <m>Y(s)</m> is found by using its partial fraction representation and referring to <xref ref="table_laplace-transforms">Table</xref>.
    We now show how the theory of complex variables can be used to systematically find the partial fraction representation.
    The first result is an extension of <xref ref="Jordan_s_Lemma">Lemma</xref> to <m>n</m> linear factors.
    The proof is left for the reader.
  </p>
  <theorem xml:id="thm_nonrepeated-factors">
    <title>Nonrepeated Linear Factors</title>
    <statement>
      <p>
        Let <m>P(s)</m> be a polynomial of degree at most <m>n-1</m>.
        If <m>Q(s)</m> has degree <m>n</m>,
        and has distinct complex roots <m>a_1,a_2,\ldots,a_n</m>,
        then Equation <xref ref="quotientPQ"/> has the representation
        <men xml:id="nonrepfact">
          Y(s) = \frac{P(s)}{(s-a_1)(s-a_2) \cdots (s-a_n)} = \sum_{k=1}^n\frac{\mathrm{Res}[Y,a_k]}{s-a_k}
        </men>.
      </p>
    </statement>
  </theorem>
  <theorem xml:id="thm_repeated-linear-factor">
    <title>A Repeated Linear Factor</title>
    <statement>
      <p>
        If <m>P(s)</m> and <m>Q(s)</m> are polynomials of degree <m>\mu</m> and <m>v</m>,
        respectively, and <m>\mu \lt v + n</m> and <m>Q(a) \ne 0</m>,
        then Equation <xref ref="quotientPQ"/> has the representation
        <men xml:id="repeatfact">
          Y(s) = \frac{P(s)}{(s-a)^nQ(s)} = \sum_{k=1}^n\frac{A_k}{(s-a)^k} +R (s)
        </men>,
        where <m>R</m> is the sum of all partial fractions that do not involve factors of the form <m>(s-a)^j</m>.
        Furthermore,
        the coefficients <m>A_k</m> can be computed with the formula
        <men xml:id="coeffPQ">
          A_k = \frac{1}{(n-k)}\lim_{s \to a}\left[\frac{d^{n-k}}{ds^{n-k}}\left(\frac{P(s)}{Q(s)}\right)\right] \text{ for }   k=1,2,\ldots,n
        </men>.
      </p>
    </statement>
  </theorem>
  <proof>
    <p>
      We employ the method of residues.
      First, multiplying both sides of Equation <xref ref="repeatfact"/> by <m>(s-a)^n</m> gives
      <me>
        \frac{P(s)}{Q(s)}=\sum\limits_{j=1}^nA_j(s-a)^{n-j}+R(s)(s-a)^n
      </me>.
      We can differentiate both sides of this equation <m>n-k</m> times to obtain
      <me>
        \frac{d^{n-k}}{ds^{n-k}}\left(\frac{P(s)}{Q(s)}\right) = \sum_{j=1}^kA_j\frac{(n-j)!}{(k-j)!}(s-a)^{k-j} + \frac{d^{n-k}}{ds^{n-k}}[R(s)(s-a)^n]
      </me>.
    </p>
    <p>
      In this equation, take the limit as <m>s \to a</m>.
      It is left as an exercise for the reader to fill in the steps to obtain
      <me>
        \lim_{s \to a}\frac{d^{n-k}}{ds^{n-k}}\left(\frac{P(s)}{Q(s)}\right) = (n-k)! A_k
      </me>.
      which establishes Equation <xref ref="coeffPQ"/>.
    </p>
  </proof>
  <example>
    <statement>
      <p>
        Let <m>Y(s) =\frac{s^3-4s+1}{s(s-1)^3}</m>.
        Find <m>\mathcal{L}^{-1}\big(Y(s)\big)</m>.
      </p>
    </statement>
    <solution>
      <p>
        From Equations <xref ref="nonrepfact"/> and <xref ref="repeatfact"/> we can write
        <me>
          \frac{s^3-4s-1}{s(s-1)^3} = \frac{A_3}{(s-1)^3} + \frac{A_2}{(s-1)^2}+\frac{A_1}{s-1}+\frac{B_1}{s}
        </me>.
        The coefficient <m>B_1</m> is found by the calculation
        <me>
          B_1 = \mathrm{Res}[Y,0] = \lim_{s \to 0}\frac{s^3-4s+1}{(s-1)^3} = -1
        </me>.
      </p>
      <p>
        The coefficients <m>A_1, \, A_2</m>,
        and <m>A_3</m> are found by using <xref ref="thm_repeated-linear-factor">Theorem</xref>.
        In this case <m>a=1</m> and <m>\frac{P(s)}{Q(s)} = \frac{s^3-4s+1}{s}</m>,
        so we get
        <md>
          <mrow>A_3 \amp = \lim_{s \to 1}\left(\frac{P(s)}{Q(s)}\right) = \lim_{s \to 1}\frac{s^3-4s+1}{s} = -2.</mrow>
          <mrow>A_2 \amp = \frac{1}{1!}\lim_{s \to 1}\frac{d}{ds}\left(\frac{P(s)}{Q(s)}\right) = \lim_{s \to 1}\left(2s-\frac{1}{s^2}\right) = 1.</mrow>
          <mrow>A_1 \amp = \frac{1}{2}\lim_{s \to 1}\frac{d^2}{ds^2}\left(\frac{P(s)}{Q(s)}\right) = \frac{1}{2}\lim_{s \to 1}\left(2+\frac{2}{s^3}\right) = 2</mrow>
        </md>.
      </p>
      <p>
        Hence, the partial fraction representation is
        <me>
          Y(s) = \frac{-2}{(s-1)^3}+\frac{1}{(s-1)^2} + \frac{2}{s-1} - \frac{1}{s}
        </me>,
        and the inverse is
        <me>
          y(t) =-t^2e^t+te^t+2e^t-1
        </me>.
      </p>
    </solution>
  </example>
  <theorem xml:id="thm_irreducible-quad-factors">
    <title>Irreducible Quadratic Factors</title>
    <statement>
      <p>
        Let <m>P</m> and <m>Q</m> be polynomials with real coefficients such that the degree of <m>P</m> is at most <m>1</m> larger than the degree of <m>Q</m>.
        If <m>T</m> does not have a factor of the form <m>(s-a)^2+b^2</m>, then
        <me>
          Y(s) = \frac{P(s)}{Q(s)} = \frac{P(s)}{\Big[(s-a)^2+b^2\Big]T(s)} = \frac{2A(s-a)-2Bb}{(s-a)^2+b^2} + R(s), \text{ where }
        </me>
        <men xml:id="AandB">
          A+iB=\frac{P(a+ib)}{Q\,'(a+ib)}
        </men>.
      </p>
    </statement>
  </theorem>
  <proof>
    <p>
      Since <m>P, \, Q</m>,
      and <m>Q'</m> have real coefficients, it follows that
      <me>
        P(a-ib) = \overline{P(a+ib)}  \text{ and }   Q'(a-ib) = \overline{Q'(a+ib)}
      </me>.
      The polynomial <m>Q</m> has simple zeros at <m>s=a\pm ib</m>,
      this implies that <m>Q'(a\pm ib) \ne 0</m>.
      Therefore, we obtain
      <men xml:id="residueY">
        \mathrm{Res}[Y,a\pm ib] = \lim_{s \to a\pm ib}\left(\frac{s-(a\pm ib)}{Q(s)-Q(a\pm ib)}P(s)\right) = \frac{P(a\pm ib)}{Q'(a\pm ib)}
      </men>,
      from which it is easy to see that
      <men xml:id="residueYconj">
        \mathrm{Res}[Y,a-ib] = \overline{\mathrm{Res}[Y,a-ib]}
      </men>.
    </p>
    <p>
      If we set <m>A+iB=</m> <m>\mathrm{Res}[Y,a+ib]</m> and use <xref ref="thm_nonrepeated-factors">Theorem</xref>
      and Equations <xref ref="AandB"/>,
      <xref ref="residueY"/>, and <xref ref="residueYconj"/>, then we find that
      <me>
        Y(s) = \frac{A+iB}{s-a-ib}+\frac{A-iB}{s-a+ib}+R(s)
      </me>.
      The first two terms on the right side of this equation are now combined to obtain
      <me>
        \frac{(A+iB)(s-a+ib)+(A-iB)(s-a-ib)}{(s-a)^2+b^2} = \frac{2A(s-a)-2Bb}{(s-a)^2+b^2}
      </me>,
      which completes the proof of the theorem.
    </p>
  </proof>
  <example>
    <statement>
      <p>
        Let <m>Y(s) = \frac{5s}{(s^2+4) (s^2+9)}</m>.
        Find <m>\mathcal{L}^{-1}\big(Y(s)\big)</m>.
      </p>
    </statement>
    <solution>
      <p>
        Here we have <m>P(s)=5s</m> and <m>Q(s)=s^4+13s^2+36</m>,
        and the roots of <m>Q(s)</m> occur at <m>0 \pm 2i</m> and <m>0 \pm 3i</m>.
        Computing the residues gives
        <md>
          <mrow>\mathrm{Res}[Y,2i] \amp = \frac{P(2i)}{Q'(2i)} = \frac{5(2i)}{4(2i)^3-26(2i)} = \frac{1}{2},  \text{ and }</mrow>
          <mrow>\mathrm{Res}[Y,3i] \amp = \frac{P(3i)}{Q'(3i)} = \frac{5(3i)}{4(3i)^3-26(3i)} = -\frac{1}{2}</mrow>
        </md>.
      </p>
      <p>
        We find that <m>A_1+iB_1=\frac{1}{2}+0i</m> and <m>A_2+iB_2=-\frac{1}{2}+0i</m>,
        which correspond to <m>a_1+ib_1=0+2i</m> and <m>a_2+ib_2=0+3i</m>,
        respectively.
        Thus we obtain
        <me>
          Y(s) = \frac{2(\frac{1}{2})(s-0) - (2)(0)(2)}{s^2+4} + \frac{2(-\frac{1}{2})(s-0)-(2)(0)(3)}{s^2+9}=\frac{s}{s^2+4}-\frac{s}{s^2+9}
        </me>,
        and the desired solution is
        <me>
          \mathcal{L}^{-1}\big(Y(s)\big) = \mathcal{L}^{-1}\left(\frac{s}{s^2+4}\right) - \mathcal{L}^{-1}\left(\frac{s}{s^2+9}\right) = \cos 2t-\cos 3t
        </me>
      </p>
    </solution>
  </example>
  <example>
    <statement>
      <p>
        Find <m>\mathcal{L}^{-1}\big(Y(s)\big)</m> if <m>Y(s) = \frac{s^3+3s^2-s+1}{s(s+1)^2(s^2+1)}</m>.
      </p>
    </statement>
    <solution>
      <p>
        The partial fraction expression for <m>Y(s)</m> has the form
        <me>
          Y(s) = \frac{D}{s}+\frac{C_1}{s+1}+\frac{C_2}{(s+1)^2} + \frac{2A(s-0) - 2B(1)}{(s-0)^2+1^2}
        </me>.
        Since the linear factor <m>s</m> is nonrepeated, we have
        <me>
          D = \mathrm{Res}[Y(s),0] = \lim_{s \to 0} \frac{s^3+3s^2-s+1}{(s+1)^2(s^2+1)} = 1
        </me>.
      </p>
      <p>
        Since the factor <m>s+1</m> is repeated, we have
        <md>
          <mrow>C_1 \amp = \mathrm{Res}[Y(s),-1]</mrow>
          <mrow>\amp = \lim_{s\to -1}\frac{d}{ds}\left(\frac{s^3+3s^2-s+1}{s(s^2+1)}\right)</mrow>
          <mrow>\amp = \lim_{s \to -1}\frac{-3s^4+4s^3-1}{s^2(s+1)^2}</mrow>
          <mrow>\amp = -2;</mrow>
          <mrow>C_2 \amp =\mathrm{Res}[(s+1) Y(s) ,-1]</mrow>
          <mrow>\amp =\lim\limits_{s \to -1}\frac{s^3+3s^2-s+1}{s(s^2+1)}</mrow>
          <mrow>\amp =-2</mrow>
        </md>.
      </p>
      <p>
        The term <m>s^2+1</m> is an irreducible quadratic,
        with roots <m>\pm i</m>, so that
        <me>
          A+iB = \mathrm{Res}[Y,i] =\lim\limits_{s \to i}\frac{s^3+3s^2-s+1}{s(s+1)^2(s+i)} = \frac{1-i}{2}
        </me>,
        and we obtain <m>A=\frac{1}{2}</m> and <m>B=-\frac{1}{2}</m>.
        Therefore,
        <md>
          <mrow>Y(s) \amp = \frac{1}{s}+\frac{-2}{s+1}+\frac{-2}{(s+1)^2} + \frac{2\frac{1}{2}(s-0)-2(-\frac{1}{2})(1)}{(s-0)^2+1^2}</mrow>
          <mrow>\amp = \frac{1}{s} - \frac{2}{s+1} - \frac{2}{(s+1)^2} + \frac{s+1}{s^2+1}</mrow>
        </md>.
      </p>
      <p>
        Now we use <xref ref="table_laplace-transforms">Table</xref> to get
        <me>
          y(t) = 1-2e^{-t}-2te^{-t} + \cos t + \sin t
        </me>
      </p>
    </solution>
  </example>
  <example>
    <statement>
      <p>
        Use Laplace transforms to solve the system
        <md>
          <mrow>y\,'(t) \amp = y(t) - x(t),  \text{ with }   y(0) = 1.</mrow>
          <mrow>x\,'(t) \amp = 5y(t) -3x(t)  \text{ with }    x(0) =2</mrow>
        </md>.
      </p>
    </statement>
    <solution>
      <p>
        Let <m>Y(s)</m> and <m>X(s)</m> denote the Laplace transforms of <m>y(t)</m> and <m>x(t)</m>,
        respectively.
        If we take the transforms of the two differential equations and get
        <md>
          <mrow>sY(s) -1 \amp = Y(s) -X(s),</mrow>
          <mrow>sX(s) -2 \amp = 5Y(s) -3X(s)</mrow>
        </md>,
        which can be written as
        <md>
          <mrow>(s-1) Y(s) +X(s) \amp = 1.</mrow>
          <mrow>5Y(s) -(s+3) X(s) \amp = -2</mrow>
        </md>.
      </p>
      <p>
        Cramer's rule can be used to solve for <m>Y(s)</m> and <m>X(s)</m>:
        <md>
          <mrow>Y(s) \amp = \frac{ \begin{vmatrix} 1 \amp  1</mrow>
          <mrow>-2 \amp  -s-3 \end{vmatrix} } { \begin{vmatrix} s-1 \amp  1</mrow>
          <mrow>5 \amp  -s-3 \end{vmatrix} } = \frac{-s-3+2}{(s-1) (-s-3) -5} = \frac{s+1}{(s+1)^2+1}</mrow>
          <mrow>X(s) \amp = \frac{ \begin{vmatrix} s-1 \amp  1</mrow>
          <mrow>5 \amp  -2 \end{vmatrix} } { \begin{vmatrix} s-1 \amp  1</mrow>
          <mrow>5 \amp  -s-3 \end{vmatrix} } = \frac{-2s+2-5}{(s-1)(-s-3)-5} = \frac{2(s+1) +1}{(s+1)^2+1}</mrow>
        </md>.
      </p>
      <p>
        The desired solution is obtained by computing the inverse transforms:
        <md>
          <mrow>y(t) \amp = e^{-t}\cos t,</mrow>
          <mrow>x(t) \amp = e^{-t}(2\cos t+\sin t) </mrow>
        </md>.
      </p>
    </solution>
  </example>
  <p>
    According to Equation <xref ref="LaplaceInverse"/> of <xref ref="sec_laplace-transform">Section</xref>,
    the inverse Laplace transform is given by the integral formula
    <me>
      f(t) = \mathcal{L}^{-1}\big(F(s)\big) = \frac{1}{2\pi i}\int_{\sigma_0-i\infty}^{\sigma_0+i\infty}F(s)e^{st}\,ds
    </me>,
    where <m>\sigma_0</m> is any suitably chosen large positive constant.
    This improper integral is a contour integral taken along the vertical line
    <m>s=\sigma_0+i\tau</m> in the complex <m>s=\sigma +i\tau</m> plane.
    We shall show how the residue theory in <xref ref="ch_residue"/> is used to evaluate it.
    Cases where the integrand has either infinitely many poles or has branch points is left for the reader to research in advanced texts.
    We state the following more elementary result.
  </p>
  <theorem xml:id="thm_inverse-laplace">
    <title>Inverse Laplace Transform</title>
    <statement>
      <p>
        Let <m>F(s) =\frac{P(s)}{Q(s)}</m>,
        where <m>P(s)</m> and <m>Q(s)</m> are polynomials of degree <m>m</m> and <m>n</m>,
        respectively, and <m>n>m</m>.
        The inverse Laplace transformation <m>F(s)</m>,
        denoted by <m>f(t)</m>, is given by
        <men xml:id="invlapform">
          f(t) = \mathcal{L}^{-1}\big(F(s)\big) = \sum \mathrm{Res}[F(s)e^{st},s_k]
        </men>,
        where the sum is taken over all of the residues of the complex function
        <m>F(s) e^{st}</m> at its poles <m>s_k</m>.
      </p>
    </statement>
  </theorem>
  <proof>
    <p>
      Let <m>\sigma_0</m> be chosen so that all the poles of
      <m>F(s) e^{st}</m> lie to the left of the vertical line <m>s=\sigma_0+i\tau</m>.
      Let <m>\Gamma_{R}</m> denote the contour consisting of the vertical line segment between the points
      <m>\sigma_0\pm iR</m> and the left semicircle <m>C_{R}:s=\sigma_0+\mathrm{Re}^{i\theta}</m>,
      where <m>\frac{\pi}{2} \le \theta \le \frac{3\pi}{2}</m>,
      as illustrated in <xref ref="fig_ch-11-27">Figure</xref>.
      A slight modification of the proof of Jordan's lemma shows that
      <me>
        \lim_{R \to +\infty}\int_{C_{R}}\frac{P(s)}{Q(s)}e^{st}\,ds = 0
      </me>.
    </p>
    <p>
      The residue theorem and above limit imply that
      <me>
        \mathcal{L}^{-1}\big(F(s)\big) = \lim_{R \to +\infty}\frac{1}{2\pi i}\int_{\Gamma_{R}}\frac{P(s)}{Q(s)} e^{st}\,ds = \sum \mathrm{Res}[F(s)e^{st}, s_k]
      </me>.
    </p>
  </proof>
  <figure xml:id="fig_ch-11-27">
    <caption>The contour <m>\Gamma_R</m>.</caption>
    <image width="73%" source="figs/ch-11/ch-11-fig-27.svg"/>
  </figure>
  <theorem>
    <title>Heaviside Expansion Theorem</title>
    <statement>
      <p>
        Let <m>P(s)</m> and <m>Q(s)</m> be polynomials of degree <m>m</m> and <m>n</m>,
        respectively, where <m>n>m</m>.
        If <m>Q(s)</m> has <m>n</m> distinct simple zeros at the points <m>s_1,s_2,\ldots,s_n</m>,
        then <m>\frac{P(s)}{Q(s)}</m> is the Laplace transform of the function <m>f(t)</m> given by
        <men xml:id="expansionform">
          f(t) = \mathcal{L}^{-1}\left(\frac{P(s)}{Q(s)}\right) = \sum_{k=1}^n\frac{P(s_k)}{Q'(s_k)}e^{s_kt}
        </men>.
      </p>
    </statement>
  </theorem>
  <proof>
    <p>
      If <m>P(s)</m> and <m>Q(s)</m> are polynomials and <m>s_k</m> is a simple zero of <m>Q(s)</m>, then
      <me>
        \mathrm{Res}[F(s) e^{st},s_k] = \lim_{s \to s_k}\frac{s-s_k}{Q(s) - Q(s_k)}P(s)e^{st} = \frac{P(s_k)}{Q'(s_k)}e^{s_kt}
      </me>.
      This outcome allows us to write the residues in Equation <xref ref="invlapform"/> in the more convenient form given in Equation <xref ref="expansionform"/>.
    </p>
  </proof>
  <example>
    <statement>
      <p>
        Find the inverse Laplace transform of the function
        <me>
          F(s) = \frac{4s+3}{s^3+2s^2+s+2}
        </me>
      </p>
    </statement>
    <solution>
      <p>
        Here we have <m>P(s)=4s+3</m> and <m>Q(s)=(s+2)(s^2+1)</m>,
        so that <m>Q</m> has simple zeros located at the points <m>s_1=-2, \, s_2=i</m>,
        and <m>s_3=-i</m>.
        Using <m>Q'(s) = 3s^2+4s+1</m>,
        calculation reveals that <m>\frac{P(-2)}{Q'(-2)}=\frac{-8+3}{12-8+1}=-1</m> and <m>\frac{P(\pm i)}{Q'(\pm i)} = \frac{\pm 4i+3}{-2\pm 4i}=\frac{1}{2}\mp i</m>.
        Applying <xref ref="expansionform">formula</xref>,
        we see that <m>f(t)</m> is given by
        <md>
          <mrow>f(t) \amp = \frac{P(-2)}{Q'(-2)}e^{-2t} + \frac{P(i)}{Q'(i)}e^{it} + \frac{P(-i)}{Q'(-i)}e^{-it}</mrow>
          <mrow>\amp = -e^{-2t}+(\frac{1}{2}-i) e^{it}+(\frac{1}{2}+i)e^{-it}</mrow>
          <mrow>\amp = -e^{-2t}+\frac{e^{it}+e^{-it}}{2}+2\frac{e^{it}-e^{-it}}{2i}</mrow>
          <mrow>\amp = -e^{-2t}+\cos t+2\sin t</mrow>
        </md>.
      </p>
    </solution>
  </example>
  <exercises xml:id="exercises_laplace-inversion">
    <title>Exercises</title>
    <exercise>
      <statement>
        <p>
          Use partial fractions to find the inverse Laplace transform of
        </p>
        <task>
          <p>
            <m>Y(s) = \frac{2s+1}{s(s-1)}</m>.
          </p>
          <solution>
            <p>
              <m>\mathcal{L}^{-1}\Big(\frac{2s+1}{s(s-1)}\Big) = -1 + 3e^t</m>.
            </p>
          </solution>
        </task>
        <task>
          <p>
            <m>Y(s) = \frac{2s^3-s^2+4s-6}{s^4}</m>.
          </p>
        </task>
        <task>
          <p>
            <m>Y(s) = \frac{4s^2-6s-12}{s(s+2)(s-2)}</m>.
          </p>
          <solution>
            <p>
              <m>\mathcal{L}^{-1}\Big(\frac{4s^2-6s-12}{s(s+2)(s-2)}\Big) = 3 + 2e^{-2t} - e^{2t}</m>.
            </p>
          </solution>
        </task>
        <task>
          <p>
            <m>Y(s) = \frac{s^3-5s^2+6s-6}{(s-2)^4}</m>.
          </p>
        </task>
        <task>
          <p>
            <m>Y(s) = \frac{2s^2+s+3}{(s+2)(s-1)^2}</m>.
          </p>
          <solution>
            <p>
              <m>\mathcal{L}^{-1}\Big(\frac{2s^2+s+3}{(s+2)(s-1)^2}\Big) = e^{-2t} + e^t + 2te^t</m>.
            </p>
          </solution>
        </task>
        <task>
          <p>
            <m>Y(s) = \frac{4-s}{s^2+4s+5}</m>.
          </p>
        </task>
      </statement>
    </exercise>
    <exercise>
      <statement>
        <p>
          Use a contour integral to find the inverse Laplace transform of
        </p>
        <task>
          <p>
            <m>Y(s) = \frac{1}{s^2+4}</m>.
          </p>
          <solution>
            <p>
              <m>\mathcal{L}^{-1}\Big(\frac{1}{s^2+4}\Big) = \frac{1}{2}\sin 2t</m>.
            </p>
          </solution>
        </task>
        <task>
          <p>
            <m>Y(s) = \frac{s+3}{(s-2)(s^2+1)}</m>.
          </p>
        </task>
      </statement>
    </exercise>
    <exercise>
      <statement>
        <p>
          Use the Heaviside Expansion Theorem to find the inverse Laplace transform of
        </p>
        <task>
          <p>
            <m>Y(s) =\frac{s^3+s^2-s+3}{s^{5}-s}</m>.
          </p>
          <solution>
            <p>
              <m>\mathcal{L}^{-1}\Big(\frac{s^3+s^2-s+3}{s^5-s}\Big) = -3+e^t+e^{-t}+\cos t+\sin t=-3+2\cosh t+\cos t+\sin t</m>.
            </p>
          </solution>
        </task>
        <task>
          <p>
            <m>Y(s) =\frac{s^3+2s^2-s+2}{s^{5}-s}</m>.
          </p>
        </task>
        <task>
          <p>
            <m>Y(s) =\frac{s^3+3s^2-s+1}{s^{5}-s}</m>.
          </p>
          <solution>
            <p>
              <m>\mathcal{L}^{-1}\Big(\frac{s^{3}+3s^2-s+1}{s^{5}-s}\Big) = -1+e^t+e^{-t}-\cos t+\sin t=-1+2\cosh t-\cos t+\sin t</m>.
            </p>
          </solution>
        </task>
        <task>
          <p>
            <m>Y(s) =\frac{s^3+s^2+s+3}{s^{5}-s}</m>.
          </p>
        </task>
      </statement>
    </exercise>
    <exercise>
      <statement>
        <p>
          Find the inverse Laplace transform of <m>Y(s) = \frac{s^3+2s^2+4s+2}{(s^2+1)(s^2+4)}</m>.
        </p>
      </statement>
      <solution>
        <p>
          <m>\mathcal{L}^{-1}\Big(\frac{s^{3}+2s^2+4s+2}{(s^2+1)(s^2+4)}\Big) = \cos t+\sin 2t</m>.
        </p>
      </solution>
    </exercise>
    <exercise>
      <statement>
        <p>
          Solve the following initial value problems.
        </p>
        <task>
          <p>
            <m>y\,''(t) + 2y\,'(t) + 5y(t) = 4e^{-t}</m>,
            with <m>y(0) = 1</m> and <m>y\,'(0) = 1</m>.
          </p>
          <solution>
            <p>
              <m>y(t) = e^{-t}+e^{-t}\sin 2t</m>.
            </p>
          </solution>
        </task>
        <task>
          <p>
            <m>y\,''(t) +y(t) = 3\sin 2t</m>,
            with <m>y(0) =0</m>, and <m>y\,'(0) = 3</m>.
          </p>
        </task>
        <task>
          <p>
            <m>y\,''(t) +4y(t) = 5e^{-t}</m>,
            with <m>y(0) =2</m> and <m>y\,'(0) = 1</m>.
          </p>
          <solution>
            <p>
              <m>y(t) = e^{-t}+\cos 2t+\sin 2t</m>.
            </p>
          </solution>
        </task>
        <task>
          <p>
            <m>y\,''(t) + 2y\,'(t) + 2y(t) = 2</m>,
            with <m>y(0) = 1</m> and <m>y\,'(0) = 1</m>.
          </p>
        </task>
        <task>
          <p>
            <m>y\,''(t) + 3y\,'(t) + 2y(t) = 2t + 5</m>,
            with <m>y(0) = 1</m> and <m>y\,'(0) = 1</m>.
          </p>
          <solution>
            <p>
              <m>y(t) = 1+t</m>.
            </p>
          </solution>
        </task>
        <task>
          <p>
            <m>y\,''(t) + 2y\,'(t) +y(t) = t</m>,
            with <m>y(0) = -1</m> and <m>y\,'(0) = 0</m>.
          </p>
        </task>
      </statement>
    </exercise>
    <exercise>
      <statement>
        <p>
          Solve the following systems of differential equations.
        </p>
        <task>
          <p>
            <m>x\,'(t) = 2y(t) - 3x(t), \, y\,'(t) = 2y(t) - 2x(t)</m>,
            with <m>x(0) = 1</m> and <m>y(0) = -1</m>.
          </p>
          <solution>
            <p>
              <m>x(t) = 2e^{-2t}-e^t</m>, and <m>y(t) = e^{-2t} - 2e^t</m>.
            </p>
          </solution>
        </task>
        <task>
          <p>
            <m>x\,'(t) = 10y(t) - 5x(t), \, y\,'(t) = y(t) - x(t)</m>,
            with <m>x(0) = 3</m> and <m>y(0) = 1</m>.
          </p>
        </task>
        <task>
          <p>
            <m>x\,'(t) = 4y(t) - 3x(t), \, y\,'(t) = y(t) -x(t)</m>,
            with <m>x(0) = -1</m> and <m>y(0) = 0</m>.
          </p>
          <solution>
            <p>
              <m>x(t) = -e^{-t} + 2te^{-t}</m>,
              and <m>y(t) = te^{-t}</m>.
            </p>
          </solution>
        </task>
        <task>
          <p>
            <m>x\,'(t) = 2x(t) +3y(t), \, y\,'(t) = 2x(t) + y(t)</m>,
            with <m>x(0) = 2</m> and <m>y(0) = 3</m>.
          </p>
        </task>
        <task>
          <p>
            <m>x\,'(t) = 8y(t) - 3x(t) + 2, \, y\,'(t) = y(t) - x(t) - 1</m>,
            with <m>x(0) = 4</m> and <m>y(0) = 2</m>.
          </p>
          <solution>
            <p>
              <m>x(t) = -2+6e^{-t}\cos 2t+6e^{-t}\sin 2t</m>,
              and <m>y(t)=-1+3e^{-t}\cos 2t</m>.
            </p>
          </solution>
        </task>
        <task>
          <p>
            <m>x\,'(t) = 4y(t) - 3x(t) + 5, \, y\,'(t) =y (t) - x(t) + 1</m>,
            with <m>x(0) =0</m> and <m>y(0) = 2</m>.
          </p>
        </task>
      </statement>
    </exercise>
  </exercises>
</section>