<section xml:id="sec_fourier-transform">
  <title>The Fourier Transform</title>
  <p>
    Let <m>U(t)</m> be a real-valued function with period <m>2\pi</m> which is piecewise continuous such that <m>U\,'(t)</m> also exists and is piecewise continuous.
    Then <m>U(t)</m> has the <em>complex Fourier series</em> representation
    <me>
      U(t) = \sum_{n=-\infty}^{\infty}c_ne^{int},  \text{ where }
    </me>
    <me>
      c_n=\frac{1}{2\pi}\int_{-\pi}^{\pi}U(t) e^{-int}\,dt  \text{ for all }   n
    </me>.
  </p>
  <p>
    The coefficients <m>\{c_nt\}</m> are complex numbers.
    Previously, we expressed <m>U(t)</m> as a real trigonometric series:
    <men xml:id="TrigSeries">
      U(t) =\frac{a_0}{2}+\sum\limits_{n=1}^{\infty}(a_n\cos nt+b_n\sin nt)
    </men>.
  </p>
  <p>
    Hence, a relationship between the coefficients is
    <md>
      <mrow>a_n=c_n+c_{-n} \amp   \text{ for }   n=0,1,2, \ldots , \text{ and }</mrow>
      <mrow>b_n=i(c_n-c_{-n}) \amp   \text{ for }   n=1,2, \ldots </mrow>
    </md>,
  </p>
  <p>
    These relations are easy to establish.
    We start by writing
    <md>
      <mrow xml:id="TrigSeries2" number="yes">U(t) \amp = c_0 + \sum_{n=1}^{\infty}c_ne^{int} + \sum_{n=1}^{\infty}c_{-n}e^{-int}</mrow>
      <mrow>\amp = c_0 + \sum_{n=1}^{\infty}c_n(\cos nt+i\sin nt) + \sum_{n=1}^{\infty}c_{-n}(\cos nt-i\sin nt)</mrow>
      <mrow>\amp = c_0 + \sum_{n=1}^{\infty}[(c_n+c_{-n}) \cos nt+i(c_n-c_{-n}) \sin nt]</mrow>
    </md>.
  </p>
  <p>
    Comparing Equation <xref ref="TrigSeries2"/> with Equation <xref ref="TrigSeries"/>, we see that <m>a_0=2c_0</m>,
    <m>a_n=c_n+c_{-n}</m>, and <m>b_n=i( c_n-c_{-n})</m>.
  </p>
  <p>
    If <m>U(t)</m> and <m>U\,'(t)</m> are piecewise continuous and have period <m>2L</m>,
    then <m>U(t)</m> has the <em>complex Fourier series</em> representation
    <men xml:id="ComplexFourier">
      U(t) = \sum_{n=-\infty}^{\infty}c_ne^{i\frac{\pi nt}{L}},  \text{ where }
    </men>
    <men xml:id="ComplexFourierC">
      c_n = \frac{1}{2L}\int_{-L}^{L}U(t) e^{-i\frac{\pi nt}{L}}\,dt  \text{ for all }   n
    </men>.
  </p>
  <p>
    We have seen how periodic functions are represented by trigonometric series.
    Many practical problems involve nonperiodic functions.
    A representation analogous to Fourier series for a nonperiodic function <m>U(t)</m> is obtained by considering the Fourier series of <m>U(t)</m> for
    <m>-L\lt t\lt L</m> and then taking the limit as <m>L \to \infty</m>.
    The result is known as the Fourier transform of <m>U(t)</m>.
  </p>
  <p>
    Start with a nonperiodic function <m>U(t)</m> and consider the periodic function <m>U_L(t)</m> with period <m>2L</m>, where
    <md>
      <mrow>U_L(t) \amp = U(t) \amp \amp  \text{ for }   -L\lt t \le L,  \text{ and }</mrow>
      <mrow>U_L(t) \amp =U_L(t+2L) \amp \amp  \text{ for all }   t</mrow>
    </md>.
  </p>
  <p>
    Then <m>U_L(t)</m> has the complex Fourier series representation
    <men xml:id="ComplexFourierL">
      U_L(t)=\sum_{n=-\infty}^{\infty}c_ne^{i\frac{\pi nt}{L}}
    </men>.
  </p>
  <p>
    We introduce some terminology to discuss the terms in Equation <xref ref="ComplexFourierL"/>, first
    <men xml:id="Frequency">
      w_n=\frac{\pi n}{L}  \text{ is called the  frequency. }
    </men>
  </p>
  <p>
    If <m>t</m> denotes time,
    then the units for <m>w_n</m> are radians per unit time.
    The set of all possible frequencies is called the
    <em>frequency spectrum, i.e.</em>,
    <me>
      \left\{\ldots ,\frac{-3\pi}{L},\frac{-2\pi}{L},\frac{-\pi}{L},\frac{\pi}{L}, \frac{2\pi}{L},\frac{3\pi}{L}, \ldots\right\}
    </me>.
  </p>
  <p>
    It is important to note that as <m>L</m> increases,
    the spectrum becomes finer and approaches a continuous spectrum of frequencies.
    It is reasonable to expect that the summation in the Fourier series for <m>U_L(t)</m> will give rise to an integral over <m>[-\infty .\infty ]</m>.
    This is stated in the following important theorem.
  </p>
  <theorem xml:id="thm_fourier-transform">
    <title>Fourier Transform</title>
    <statement>
      <p>
        Let <m>U(t)</m> and <m>U\,'(t)</m> be piecewise continuous, and
        <me>
          \int_{-\infty}^{\infty}\left| U(t) \right| dt\lt M
        </me>,
        for some positive constant <m>M</m>.
        The Fourier transform <m>F(w)</m> of <m>U(t)</m> is defined as
        <men xml:id="FourierTransform">
          F(w) = \frac{1}{2\pi}\int\nolimits_{-\infty}^{\infty}U(t)e^{-iwt}\,dt
        </men>.
      </p>
      <p>
        At points of continuity, <m>U(t)</m> has the integral representation
        <me>
          U(t) = \int\nolimits_{-\infty}^{\infty}F(w)e^{iwt}\,dw
        </me>.
        and at a point <m>t=a</m> of discontinuity of <m>U</m>,
        the integral converges to <m>\frac{U(a^-)+U(a^+)}{2}</m>.
      </p>
    </statement>
  </theorem>
  <p>
    Note: It is common to express the fact that <m>U</m> is transformed into <m>F</m> by using the operator notation
    <me>
      \mathrm{F}\big(U(t)\big)=F(w)
    </me>
  </p>
  <proof>
    <p>
      Set <m>\Delta w_n=w_{n+1}-w_n=\frac{\pi}{L}</m> and <m>\frac{1}{2L}=\frac{1}{2\pi}\Delta w_n</m>.
      These quantities are used in conjunction with Equations <xref ref="ComplexFourier"/>, <xref ref="ComplexFourierC"/>,
      <xref ref="ComplexFourierL"/> and the frequency in <xref ref="Frequency"/> to obtain
      <md>
        <mrow xml:id="ComplexFourierL2" number="yes">U_L(t) \amp = \sum_{n=-\infty}^{\infty}\left[\frac{1}{2L} \int_{-L}^{L}U(t) e^{-iw_nt}\,dt\right] e^{iw_nt}</mrow>
        <mrow>\amp = \sum\limits_{n=-\infty}^{\infty}\left[\frac{1}{2\pi}\int_{-L}^{L}U(t) e^{-iw_nt}\,dt\right] e^{iw_nt}\Delta w_n</mrow>
      </md>.
    </p>
    <p>
      If we define <m>F_L(w)</m> by
      <me>
        F_L(w) = \frac{1}{2\pi}\int_{-L}^{L}U(t)e^{-iwt}\,dt
      </me>,
      then Equation <xref ref="ComplexFourierL2"/> can be written as
      <men xml:id="ComplexFourierL3">
        U_L(t) = \sum_{n=-\infty}^{\infty}F_L(w_n)e^{iw_nt}\Delta w_n
      </men>.
    </p>
    <p>
      As <m>L</m> gets large,
      <m>F_L(w_n)</m> approaches <m>F(w_n)</m> and <m>\Delta w_n</m> tends to zero.
      Thus the limit on the right-hand side of Equation <xref ref="ComplexFourierL3"/> can be viewed as an integral.
      This substantiates the Fourier integral representation
      <me>
        U(t) = \int_{-\infty}^{\infty}F(w)e^{iwt}dw
      </me>.
      A more rigorous proof of this fact can be found in advanced texts.
    </p>
  </proof>
  <p>
    The following table depicts some important properties of the Fourier transform.
  </p>
  <table xml:id="table_fourier-transform-properties">
    <title>Important Properties of the Fourier Transform</title>
    <tabular>
      <row bottom="minor">
        <cell></cell>
        <cell></cell>
      </row>
      <row>
        <cell>Linearity</cell>
        <cell><m>\mathrm{F}\big(aU_1(t) + bU_2(t)\big) =a\,\mathrm{F}(U_1(t)) +b\,\mathrm{F}\big(U_2(t)\big)</m>;</cell>
      </row>
      <row>
        <cell>\hdashline
          Symmetry</cell>
        <cell>If <m>\mathrm{F}\big(U(t)\big)=F(w)</m>, then <m>\mathrm{F}\big(F(t)\big) = \frac{1}{2\pi}U(-w)</m>;</cell>
      </row>
      <row>
        <cell>\hdashline
          Time scaling</cell>
        <cell><m>\mathrm{F}(U(at)) = \frac{1}{|a|}F(\frac{w}{a})</m>;</cell>
      </row>
      <row>
        <cell>\hdashline
          Time shifting</cell>
        <cell><m>\mathrm{F}(U(t-t_0)) = e^{-it_0w}F(w)</m>;</cell>
      </row>
      <row>
        <cell>\hdashline
          Frequency shifting</cell>
        <cell><m>\mathrm{F}\big(e^{-iw_0t}U(t)\big) = F(w-w_0)</m>;</cell>
      </row>
      <row>
        <cell>\hdashline
          Time differentiation</cell>
        <cell><m>\mathrm{F}\big(U\,'(t)\big) = iwF(w)</m>;</cell>
      </row>
      <row>
        <cell>\hdashline
          Frequency differentiation</cell>
        <cell><m>\frac{d^nF(w)}{dw^n} = \mathrm{F}\big((-it)^nU(t)\big)</m>;</cell>
      </row>
      <row>
        <cell>\hdashline
          Moment Theorem</cell>
        <cell>If <m>M_n = \int_{-\infty}^{\infty}t^nU(t)\,dt</m>, then <m>(-i)^nM_n = 2\pi F^{(n)}(0)</m>.</cell>
      </row>
      <row bottom="minor">
        <cell></cell>
        <cell></cell>
      </row>
    </tabular>
  </table>
  <example xml:id="ex_10_5">
    <statement>
      <p>
        Show that <m>F\big(e^{-|t|}\big) = \frac{1}{\pi(1+w^2)}</m>.
      </p>
    </statement>
    <solution>
      <p>
        Using <xref ref="FourierTransform">formula</xref> we obtain
        <md>
          <mrow>F(w) \amp =\frac{1}{2\pi}\int\nolimits_{-\infty}^{\infty}e^{-\left| t\right| }e^{-iwt}\,dt</mrow>
          <mrow>\amp = \frac{1}{2\pi}\int\nolimits_{-\infty}^{0}e^{(1-iw)t}\,dt + \frac{1}{2\pi}\int_0^{\infty}e^{(-1-iw) t}\,dt</mrow>
          <mrow>\amp = \frac{1}{2\pi (1-iw)}e^{(1-iw) t}\bigg|_{t=-\infty}^{t=0}+\frac{1}{2\pi (-1-iw)}e^{(-1-iw) t} \bigg|_{t=0}^{t=\infty}.</mrow>
          <mrow>\amp = \frac{1}{2\pi (1-iw)}+\frac{1}{2\pi (1+iw)}</mrow>
          <mrow>\amp = \frac{1}{\pi (1+w^2)}</mrow>
        </md>.
      </p>
    </solution>
  </example>
  <example>
    <statement>
      <p>
        Show that <m>\mathrm{F}\big(\frac{1}{1+t^2}\big) = \frac{1}{2}e^{-|w|}</m>.
      </p>
    </statement>
    <solution>
      <p>
        Using the result of <xref ref="ex_10_5">Example</xref>
        and the symmetry property and the symmetry property, we obtain
        <me>
          \mathrm{F}\left(\frac{1}{\pi (1+t^2)}\right) = \frac{1}{2\pi}e^{-|-w|} = \frac{1}{2\pi}e^{-|w|}
        </me>.
        By the linearity property, with each term is multiplied by <m>\pi</m>, we get
        <me>
          \mathrm{F}\left(\frac{1}{1+t^2}\right) = \frac{1}{2}e^{-|w|}
        </me>
      </p>
    </solution>
  </example>
  <exercises xml:id="exercises_fourier-transform">
    <title>Exercises</title>
    <exercise>
      <statement>
        <p>
          Find <m>\mathfrak{F}\big(U(t)\big)</m> for each of the following:
        </p>
        <task xml:id="ex_12_1a">
          <p>
            <m>U(t) = \begin{cases}1 \amp \text{ for } |t| \lt 1,\\ 0 \amp \text{ for } |t| > 1. \end{cases}</m>
          </p>
          <solution>
            <p>
              <m>\mathfrak{F}\big(U(t)\big) =\frac{\sin(w)}{\pi w}</m>.
            </p>
          </solution>
        </task>
        <task xml:id="ex_12_1b">
          <p>
            <m>U(t) = \begin{cases}1-|t| \amp \text{ for } |t| \le 1,\\ 0 \amp \text{ for } |t|>1. \end{cases}</m>
          </p>
          <solution>
            <p>
              <m>\mathfrak{F}\big(U(t)\big) =\frac{1-\cos(w)}{\pi w^2}=\frac{2\sin^2(\frac{w}{2})}{\pi w^2}</m>.
            </p>
          </solution>
        </task>
      </statement>
    </exercise>
    <exercise xml:id="ex_12_2">
      <statement>
        <p>
          Let <m>U(t) = \begin{cases}\sin t \amp \text{ for } |t| \le \pi,\\ \;\;\, 0 \amp \text{ for } |t| > \pi. \end{cases}</m> Show that <m>\mathfrak{F}\big(U(t)\big) =\frac{i\sin \pi w}{\pi (1-w^2)}</m>.
        </p>
      </statement>
    </exercise>
    <exercise>
      <statement>
        <p>
          Use the symmetry and linearity properties and the result of <xref ref="ex_12_1a">Exercise</xref> to show that
          <me>
            \mathfrak{F}\left(\frac{\sin t}{t}\right) = \begin{cases}\frac{1}{2} \amp  \text{ for }   |w| \lt  1,\\ 0 \amp  \text{ for }   |w| > 1. \end{cases}
          </me>
        </p>
      </statement>
    </exercise>
    <exercise xml:id="ex_12_3">
      <statement>
        <p>
          Let <m>U(t) =e^{-\frac{t^2}{2}}</m>.
          Show that <m>\mathfrak{F}\big(U(t)\big) = \frac{1}{\sqrt{2\pi}}e^{-\frac{w^2}{2}}</m>. \hint{Use the integral definition and combine the terms in the exponent,
          then complete the square and use the fact that <m>\int\nolimits_{-\infty}^{\infty}e^{-\frac{r^2}{2}}\,dt=\sqrt{2\pi}</m>.}
        </p>
      </statement>
    </exercise>
    <exercise>
      <statement>
        <p>
          Use the time scaling property and the example in the text to show that
          <me>
            \mathfrak{F}(e^{-a|t|}) =\frac{|a|}{\pi(a^2+w^2)}
          </me>
        </p>
      </statement>
    </exercise>
    <exercise>
      <statement>
        <p>
          Use the symmetry and linearity properties and the result of <xref ref="ex_12_2">Exercise</xref> to show that
          <me>
            \mathfrak{F}\left(\frac{i\sin \pi t}{1-t^2}\right) = \begin{cases}\frac{i\sin w}{2} \amp  \text{ for }  |w| \le \pi,\\ 0 \amp  \text{ for }   |w| > \pi. \end{cases}
          </me>
        </p>
      </statement>
    </exercise>
    <exercise>
      <statement>
        <p>
          Use the time differentiation property and the result of <xref ref="ex_12_3">Exercise</xref> to show that
          <me>
            \mathfrak{F}\left(te^{-\frac{r^2}{2}}\right) =\frac{-iwe^{-\frac{w^2}{2}}}{\sqrt{2\pi}}
          </me>
        </p>
      </statement>
    </exercise>
    <exercise>
      <statement>
        <p>
          Use the symmetry and linearity properties and the results of <xref ref="ex_12_1b">Exercise</xref> to show that
          <me>
            F\left(\frac{\sin^2\frac{t}{2}}{t^2}\right) = \begin{cases}\frac{1-|w|}{4\pi} \amp  \text{ for }   |w| \le 1, \\ 0 \amp  \text{ for }   |w| >1. \end{cases}
          </me>
        </p>
      </statement>
    </exercise>
    <exercise>
      <statement>
        <p>
          Write a report on the Fourier transform.
          Discuss some of the ideas you found in the literature that are not mentioned in the text.
        </p>
      </statement>
    </exercise>
  </exercises>
</section>